infinité ok, reste du TODO

src/Lustre/Denot/InftyProof.v
@@ -17,12 +17,28 @@ Require Import SDfuns.
 Require Import Denot.
 Require Import Infty.
 Require Import Cpo_ext.
+Import List.
 
-(** ** Proof of the determinism of the coinductive semantics
-    We can proove that the semantics of a causal program are deterministic:
-    That is, a node always return the same output for a given input.
- *)
-Module Type LSEMDETERMINISM
+(* TODO: move *)
+Lemma In_list_pair_l :
+  forall {A B} (l : list (A*B)) x y,
+    In (x,y) l -> In x (map fst l).
+Proof.
+  induction l; simpl; firstorder; subst; auto.
+Qed.
+
+(* TODO: move if used *)
+Lemma Forall_In :
+  forall {A} (P : A -> Prop) l x,
+    Forall P l ->
+    In x l ->
+    P x.
+Proof.
+  setoid_rewrite Forall_forall.
+  auto.
+Qed.
+
+Module Type LDENOTINF
        (Import Ids   : IDS)
        (Import Op    : OPERATORS)
        (Import OpAux : OPERATORS_AUX Ids Op)
@@ -33,1639 +49,600 @@ Module Type LSEMDETERMINISM
        (Import LCA   : LCAUSALITY Ids Op OpAux Cks Senv Syn)
        (Import Lord  : LORDERED Ids Op OpAux Cks Senv Syn)
        (Import CStr  : COINDSTREAMS Ids Op OpAux Cks)
-       (* (Import Sem   : LSEMANTICS Ids Op OpAux Cks Senv Syn Lord CStr) *)
        (Import Den   : LDENOT     Ids Op OpAux Cks Senv Syn Lord CStr).
 
+  Section node_inf.
 
-  Import List.
+  Context {PSyn : block -> Prop}.
+  Context {prefs : PS.t}.
+  Variable (G : @global PSyn prefs).
+  (* Variable Γ : static_env. *)
 
-  (* (** Induction hypothesis over the program *) *)
-  (* Definition det_nodes {PSyn prefs} (G : @global PSyn prefs) := forall f n ins1 ins2 outs1 outs2, *)
-  (*     Forall2 (EqStN n) ins1 ins2 -> *)
-  (*     sem_node G f ins1 outs1 -> *)
-  (*     sem_node G f ins2 outs2 -> *)
-  (*     Forall2 (EqStN n) outs1 outs2. *)
+  (* Selon Basile, il ne serait pas difficile de modifier l'élaboration
+     de sorte à ce que la propritété suivante soit vérifiée pour les nœuds
+     sans blocs. En attendant, on la suppose. *)
+  Hypothesis HasCausInj :
+    forall Γ x cx, HasCaus Γ x cx -> x = cx.
 
-  (* Lemma det_nodes_ins {PSyn prefs} : forall (G : @global PSyn prefs) f ins outs1 outs2, *)
-  (*     det_nodes G -> *)
-  (*     sem_node G f ins outs1 -> *)
-  (*     sem_node G f ins outs2 -> *)
-  (*     EqSts outs1 outs2. *)
-  (* Proof. *)
-  (*   intros * Hdet Hsem1 Hsem2. *)
-  (*   eapply EqStN_EqSts; intros. *)
-  (*   eapply Hdet. 2,3:eauto. *)
-  (*   eapply Forall2_same, Forall_forall; intros. reflexivity. *)
-  (* Qed. *)
-
-  Section sem_equation_det.
-    Context {PSyn : block -> Prop}.
-    Context {prefs : PS.t}.
-    Variable (G : @global PSyn prefs).
-
-    (* Hypothesis HdetG : det_nodes G. *)
-
-    Variable Γ : static_env.
-
-    Definition inf_var_inv n (env : DS_prod SI) : ident -> Prop :=
-      fun cx => forall x,
-          (HasCaus Γ x cx ->
-           is_cons (nrem n (env x))).
-
-    Definition inf_exp_inv n env bs : exp -> nat -> Prop :=
-      fun e k =>
-        wt_exp G Γ e ->
-        restr_exp e ->
-        is_cons (nrem n (get_nth (denot_exp e env bs) k)).
-
-    Lemma P_exps_inf_exp_inv : forall n env bs es k,
-        Forall (wt_exp G Γ) es ->
-        Forall restr_exp es ->
-        P_exps (inf_exp_inv n env bs) es k ->
-        is_cons (nrem n (get_nth (denot_exps es env bs) k)).
-    Proof.
-      induction es as [| e es]; intros * Hwt Hr Hp; inv Hwt; simpl.
-      inv Hp.
-      inv Hr; inv Hp.
-      - (* now *)
-        setoid_rewrite denot_exps_eq.
-        rewrite nprod_app_nth1; auto.
-      - (* later *)
-        setoid_rewrite denot_exps_eq.
-        rewrite nprod_app_nth2; auto.
-    Qed.
-
-    (* Lemma Forall2Brs_det_exp_inv : forall n H1 H2 bs1 bs2 es k ss1 ss2, *)
-    (*     k < length ss1 -> *)
-    (*     Forall (fun es => Forall (wt_exp G Γ) (snd es)) es -> *)
-    (*     Forall (fun es => P_exps (det_exp_inv n H1 H2 bs1 bs2) (snd es) k) es -> *)
-    (*     Forall2Brs (sem_exp G H1 bs1) es ss1 -> *)
-    (*     Forall2Brs (sem_exp G H2 bs2) es ss2 -> *)
-    (*     Forall2 (fun xs1 xs2 => EqStN n (snd xs1) (snd xs2)) (nth k ss1 []) (nth k ss2 []). *)
-    (* Proof. *)
-    (*   induction es; intros * Hlen Hwt Hp Hsem1 Hsem2; *)
-    (*     inv Hwt; inv Hsem1; inv Hsem2; simpl; inv Hp. *)
-    (*   { eapply Forall_forall in H; [|eapply nth_In]. rewrite H. 2:auto. *)
-    (*     destruct (Compare_dec.dec_lt k (length ss2)). *)
-    (*     eapply Forall_forall in H0; [|eapply nth_In]. rewrite H0. 2:auto. constructor. *)
-    (*     erewrite nth_overflow; auto. lia. *)
-    (*   } *)
-    (*   eapply P_exps_det_exp_inv in H9 as Heq1. 3:eauto. 2,3:eauto. *)
-    (*   eapply IHes in H11 as Heq2. 3-5:eauto. *)
-    (*   2:{ eapply Forall3_length in H8 as (?&?). congruence. } *)
-    (*   assert (length (concat vs1) = length (concat vs0)) as Hlen0. *)
-    (*   { eapply sem_exps_numstreams in H5; eauto with ltyping. *)
-    (*     eapply sem_exps_numstreams in H9; eauto with ltyping. congruence. } *)
-    (*   clear - Hlen Hlen0 H8 H12 Heq1 Heq2. *)
-    (*   eapply Forall3_forall3 in H8 as (?&?&?). *)
-    (*   eapply Forall3_forall3 in H12 as (?&?&?). *)
-    (*   erewrite H1 at 1; try reflexivity. *)
-    (*   erewrite H4; try reflexivity. *)
-    (*   constructor; eauto. *)
-    (*   1,2:congruence. *)
-    (* Qed. *)
-
-    Section Forall_Nprod.
-
-      Variable P : DS (sampl value) -> Prop.
-
-      Definition forall_nprod {n} (np : nprod n) : Prop.
-        induction n as [|[]]; simpl in *.
-        - exact True.
-        - exact (P np).
-        - exact (P (fst np) /\ IHn (snd np)).
-      Defined.
-
-      Lemma forall_nprod_skip :
-        forall {n} (np : nprod (S n)),
-          forall_nprod np ->
-          forall_nprod (nprod_skip np).
-      Proof.
-        intros * Hnp.
-        destruct n.
-        - now simpl.
-        - destruct Hnp. auto.
-      Qed.
-
-      Lemma forall_nprod_k :
-        forall {n} (np : nprod n),
-          (forall k, k < n -> P (get_nth np k)) ->
-          forall_nprod np.
-      Proof.
-        induction n as [|[]]; intros * Hk.
-        - constructor.
-        - apply (Hk O); auto.
-        - split.
-          + apply (Hk O); auto with arith.
-          + apply IHn; intros.
-            change (snd np) with (nprod_skip np).
-            rewrite get_nth_skip; auto with arith.
-      Qed.
-
-      Lemma forall_nprod_k' :
-        forall {n} (np : nprod n),
-          forall_nprod np ->
-          (forall k, k < n -> P (get_nth np k)).
-      Proof.
-        induction n as [|[]]; intros * Hk.
-        - lia.
-        - intros.
-          assert (k = O) by lia; subst.
-          now simpl in Hk.
-        - intros.
-          specialize (IHn (nprod_skip np)).
-          setoid_rewrite get_nth_skip in IHn.
-          destruct k. { destruct Hk; auto. }
-          apply IHn; auto using forall_nprod_skip with arith.
-      Qed.
-
-      (* Lemma forall_nprod_Oeq_compat : *)
-      (*   forall {n} (np np' : nprod n), *)
-      (*     np == np' -> *)
-      (*     forall_nprod np <-> forall_nprod np'. *)
-      (* Proof. *)
-      (*   intros * Heq. *)
-      (*   split; intro Hf. *)
-      (*   - apply forall_nprod_k; intros. *)
-      (*     rewrite <- Heq. *)
-      (*     auto using forall_nprod_k'. *)
-      (*   - apply forall_nprod_k; intros. *)
-      (*     rewrite Heq. *)
-      (*     auto using forall_nprod_k'. *)
-      (* Qed. *)
-
-      (* Add Parametric Morphism {n} : forall_nprod *)
-      (*     with signature (@Oeq (nprod n)) ==> iff as forall_nprod_compat_morph. *)
-      (* Proof. *)
-      (*   exact (forall_nprod_Oeq_compat). *)
-      (* Qed. *)
-
-      Lemma forall_nprod_app :
-        forall {n m} (np : nprod n) (mp : nprod m),
-          forall_nprod np ->
-          forall_nprod mp ->
-          forall_nprod (nprod_app np mp).
-      Proof.
-        intros * Hnp Hmp.
-        apply forall_nprod_k.
-        intros * Hk.
-        destruct (Nat.lt_ge_cases k n).
-        - rewrite nprod_app_nth1; auto using forall_nprod_k'.
-        - rewrite nprod_app_nth2; auto.
-          apply forall_nprod_k'; auto; lia.
-      Qed.
-
-      Lemma forall_nprod_lift2 :
-        forall (f : forall A, DS (sampl A) -C-> DS (sampl A) -C-> DS (sampl A)),
-          (forall x y, P x -> P y -> P (f _ x y)) ->
-          forall {n} (np np' : nprod n),
-          forall_nprod np ->
-          forall_nprod np' ->
-          forall_nprod (lift2 f np np').
-      Proof.
-        intros f Hf.
-        induction n as [|[]]; intros * H H'; auto.
-        simpl in *; auto.
-        destruct np,np',H,H'.
-        rewrite lift2_simpl.
-        split; simpl in *; auto .
-        now apply IHn.
-      Qed.
-
-    End Forall_Nprod.
-
-    Lemma numstreams_annots :
-      forall es, list_sum (map numstreams es) = length (annots es).
-    Proof.
-      induction es; simpl; auto.
-      rewrite app_length; f_equal; auto.
-      rewrite <- length_typeof_numstreams, typeof_annot.
-      now rewrite map_length.
-    Qed.
-
-    Lemma P_exps_inf_exp_inv_all : forall n env bs es,
-        Forall (wt_exp G Γ) es ->
-        Forall restr_exp es ->
-        (forall k, k < length (annots es) -> P_exps (inf_exp_inv n env bs) es k) ->
-        forall_nprod (fun s => is_cons (nrem n s)) (denot_exps es env bs).
-    Proof.
-      intros * Hwt Hr Hks.
-      rewrite <- numstreams_annots in Hks.
-      induction es; simpl; auto.
-      apply forall_nprod_k.
-      intros.
-      eapply P_exps_inf_exp_inv in Hks; eauto.
-    Qed.
-
-    Lemma EqSts_mask : forall k r ss1 ss2,
-        EqSts ss1 ss2 ->
-        EqSts (map (maskv k r) ss1) (map (maskv k r) ss2).
-    Proof.
-      unfold EqSts.
-      intros * Heq.
-      rewrite Forall2_map_1, Forall2_map_2.
-      eapply Forall2_impl_In; [|eauto]; intros ?? _ _ Hab.
-      now rewrite Hab.
-    Qed.
-
-    Lemma EqSts_unmask : forall r ss1 ss2,
-        (forall k, EqSts (map (maskv k r) ss1) (map (maskv k r) ss2)) ->
-        EqSts ss1 ss2.
-    Proof.
-      intros * Heq.
-      assert (length ss1 = length ss2) as Hlen.
-      { specialize (Heq O). eapply Forall2_length in Heq.
-        now repeat rewrite map_length in Heq. }
-      eapply Forall2_forall2. split; auto; intros ????? Hl ??; subst.
-      eapply EqSt_unmask. intros.
-      specialize (Heq k). eapply Forall2_forall2 in Heq as (_&Heq).
-      eapply Heq; eauto.
-      rewrite map_length; eauto.
-      1,2:rewrite map_nth; reflexivity.
-    Qed.
-
-    (** We first establish the determinism of all the coinductive operators,
-        as well as the expression semantics.
-        We show that they are deterministic "up-to-n" : that is they preserve
-        the equality "up-to-n".
-        Proving this for any n is stronger than just proving that they output the
-        same stream for the same input, as we can use `EqStN_EqSt` to rewrite
-        the conclusion and hypotheses.
-    *)
-
-    Hint Constructors EqStN : core.
-
-    Lemma const_detn : forall n bs1 bs2 c,
-        EqStN n bs1 bs2 ->
-        EqStN n (const bs1 c) (const bs2 c).
-    Proof.
-      induction n; intros * Hbs; auto.
-      inv Hbs. do 2 rewrite const_Cons.
-      constructor; eauto.
-    Qed.
-
-    Lemma enum_detn : forall n bs1 bs2 c,
-        EqStN n bs1 bs2 ->
-        EqStN n (enum bs1 c) (enum bs2 c).
-    Proof.
-      induction n; intros * Hbs; auto.
-      inv Hbs. rewrite (unfold_Stream (enum (_ ⋅ xs1) _)), (unfold_Stream (enum (_ ⋅ xs2) _)).
-      constructor; eauto.
-    Qed.
-
-    Lemma lift1_detn : forall n op ty xs1 xs2 ys1 ys2,
-        EqStN n xs1 xs2 ->
-        lift1 op ty xs1 ys1 ->
-        lift1 op ty xs2 ys2 ->
-        EqStN n ys1 ys2.
-    Proof.
-      induction n; intros * Heq Hl1 Hl2; auto.
-      inv Heq; inv Hl1; inv Hl2; constructor; eauto.
-      rewrite H2 in H3. now inv H3.
-    Qed.
-
-    (* Lemma lift2_detn : forall n op ty1 ty2 xs11 xs12 xs21 xs22 ys1 ys2, *)
-    (*     EqStN n xs11 xs21 -> *)
-    (*     EqStN n xs12 xs22 -> *)
-    (*     lift2 op ty1 ty2 xs11 xs12 ys1 -> *)
-    (*     lift2 op ty1 ty2 xs21 xs22 ys2 -> *)
-    (*     EqStN n ys1 ys2. *)
-    (* Proof. *)
-    (*   induction n; intros * Heq1 Heq2 Hl1 Hl2; auto. *)
-    (*   inv Heq1; inv Heq2; inv Hl1; inv Hl2; constructor; eauto. *)
-    (*   rewrite H6 in H8. now inv H8. *)
-    (* Qed. *)
-
-    (* Corollary fby_detn : forall n xs1 xs2 ys1 ys2 zs1 zs2, *)
-    (*     EqStN n xs1 xs2 -> *)
-    (*     EqStN n ys1 ys2 -> *)
-    (*     fby xs1 ys1 zs1 -> *)
-    (*     fby xs2 ys2 zs2 -> *)
-    (*     EqStN n zs1 zs2. *)
-    (* Proof. *)
-    (*   induction n; intros * Heq1 Heq2 Hfby1 Hfby2; inv Heq1; inv Heq2; *)
-    (*     inv Hfby1; inv Hfby2; constructor; auto. eauto. *)
-    (*   clear IHn. revert y xs0 xs1 xs3 xs2 rs rs0 H1 H2 H6 H7. *)
-    (*   induction n; intros * Heq1 Heq2 Hfby1 Hfby2; inv Heq1; inv Heq2; *)
-    (*     inv Hfby1; inv Hfby2; constructor; eauto. *)
-    (* Qed. *)
-
-    (* Lemma arrow_detn : forall n xs1 xs2 ys1 ys2 zs1 zs2, *)
-    (*     EqStN n xs1 xs2 -> *)
-    (*     EqStN n ys1 ys2 -> *)
-    (*     arrow xs1 ys1 zs1 -> *)
-    (*     arrow xs2 ys2 zs2 -> *)
-    (*     EqStN n zs1 zs2. *)
-    (* Proof. *)
-    (*   induction n; intros * Heq1 Heq2 Hfby1 Hfby2; inv Heq1; inv Heq2; *)
-    (*     inv Hfby1; inv Hfby2; constructor; auto. eauto. *)
-    (*   clear IHn. revert xs0 xs1 xs3 xs2 rs rs0 H1 H2 H6 H7. *)
-    (*   induction n; intros * Heq1 Heq2 Hfby1 Hfby2; inv Heq1; inv Heq2; *)
-    (*     inv Hfby1; inv Hfby2; constructor; eauto. *)
-    (* Qed. *)
-
-    (* Lemma when_detn : forall n k xs1 xs2 ys1 ys2 zs1 zs2, *)
-    (*     EqStN n xs1 xs2 -> *)
-    (*     EqStN n ys1 ys2 -> *)
-    (*     when k xs1 ys1 zs1 -> *)
-    (*     when k xs2 ys2 zs2 -> *)
-    (*     EqStN n zs1 zs2. *)
-    (* Proof. *)
-    (*   induction n; intros * Heq1 Heq2 Hwhen1 Hwhen2; inv Heq1; inv Heq2; auto. *)
-    (*   inv Hwhen1; inv Hwhen2; constructor; eauto. *)
-    (*   1,2:congruence. *)
-    (* Qed. *)
-
-    Lemma merge_detn : forall n cs1 cs2 xss1 xss2 ys1 ys2,
-        map fst xss1 = map fst xss2 ->
-        NoDupMembers xss1 ->
-        EqStN n cs1 cs2 ->
-        Forall2 (fun xs1 xs2 => EqStN n (snd xs1) (snd xs2)) xss1 xss2 ->
-        merge cs1 xss1 ys1 ->
-        merge cs2 xss2 ys2 ->
-        EqStN n ys1 ys2.
-    Proof.
-      induction n; intros * Hfst Hnd Heq1 Heq2 Hmerge1 Hmerge2; inv Heq1; auto.
-      inv Hmerge1; inv Hmerge2; constructor; eauto.
-      1,3:eapply IHn. 5,6,11,12:eauto. 1-8:eauto.
-      1,4:erewrite 2 map_map, map_ext with (l:=xss1), map_ext with (l:=xss2); eauto; intros (?&?); auto.
-      1,3:erewrite fst_NoDupMembers, map_map, map_ext, <-fst_NoDupMembers; eauto; intros (?&?); auto.
-      1,2:(rewrite Forall2_map_1, Forall2_map_2; eapply Forall2_impl_In; [|eauto];
-           intros (?&?) (?&?) _ _ Heq; inv Heq; simpl in *; subst; auto).
-      clear - Hfst Hnd Heq2 H3 H5. unfold EqSts in *.
-      induction Heq2; inv H3; inv H5; inv Hnd; simpl in *; inv Hfst; auto.
-      - destruct y, H1, H2; subst; simpl in *.
-        rewrite <-H1, <-H3. inv H; auto.
-      - exfalso. destruct y, H1; subst; simpl in *.
-        eapply H4. rewrite fst_InMembers, H6, <-fst_InMembers.
-        simpl_Exists; subst; eauto using In_InMembers.
-      - exfalso. destruct y, H2; subst; simpl in *.
-        eapply H4. rewrite fst_InMembers, <-fst_InMembers.
-        simpl_Exists; subst; eauto using In_InMembers.
-    Qed.
-
-    Lemma case_detn : forall n cs1 cs2 xss1 xss2 ys1 ys2 ds1 ds2,
-        map fst xss1 = map fst xss2 ->
-        NoDupMembers xss1 ->
-        EqStN n cs1 cs2 ->
-        Forall2 (fun xs1 xs2 => EqStN n (snd xs1) (snd xs2)) xss1 xss2 ->
-        (forall d1 d2, ds1 = Some d1 -> ds2 = Some d2 -> EqStN n d1 d2) ->
-        case cs1 xss1 ds1 ys1 ->
-        case cs2 xss2 ds2 ys2 ->
-        EqStN n ys1 ys2.
-    Proof.
-      induction n; intros * Hfst Hnd Heq1 Heq2 Heq3 Hcase1 Hcase2; inv Heq1; auto.
-      inv Hcase1; inv Hcase2.
-      - econstructor; eauto.
-        eapply IHn. 6,7:eauto. 1-5:intros; eauto.
-        erewrite 2 map_map, map_ext with (l:=xss1), map_ext with (l:=xss2); eauto; intros (?&?); auto.
-        erewrite fst_NoDupMembers, map_map, map_ext, <-fst_NoDupMembers; eauto; intros (?&?); auto.
-        (rewrite Forall2_map_1, Forall2_map_2; eapply Forall2_impl_In; [|eauto];
-           intros (?&?) (?&?) _ _ Heq; inv Heq; simpl in *; subst; auto).
-        eapply option_map_inv in H as (?&?&?); subst.
-        eapply option_map_inv in H6 as (?&?&?); subst.
-        specialize (Heq3 _ _ eq_refl eq_refl). inv Heq3; auto.
-      - econstructor; eauto.
-        + clear - Hfst Hnd Heq2 H8 H12. unfold EqSts in *.
-          induction Heq2; inv H8; inv H12; inv Hnd; simpl in *; inv Hfst; auto.
-          * destruct y, H1, H2; subst; simpl in *.
-            rewrite <-H1, <-H3. inv H; auto.
-          * exfalso. destruct y, H1; subst; simpl in *.
-            eapply H4. rewrite fst_InMembers, H6, <-fst_InMembers.
-            simpl_Exists; subst; eauto using In_InMembers.
-          * exfalso. destruct y, H2; subst; simpl in *.
-            eapply H4. rewrite fst_InMembers, <-fst_InMembers.
-            simpl_Exists; subst; eauto using In_InMembers.
-        + eapply IHn. 6,7:eauto. 1-5:intros; eauto.
-          erewrite 2 map_map, map_ext with (l:=xss1), map_ext with (l:=xss2); eauto; intros (?&?); auto.
-          erewrite fst_NoDupMembers, map_map, map_ext, <-fst_NoDupMembers; eauto; intros (?&?); auto.
-          (rewrite Forall2_map_1, Forall2_map_2; eapply Forall2_impl_In; [|eauto];
-           intros (?&?) (?&?) _ _ Heq; inv Heq; simpl in *; subst; auto).
-          eapply option_map_inv in H as (?&?&?); subst.
-          eapply option_map_inv in H0 as (?&?&?); subst.
-          specialize (Heq3 _ _ eq_refl eq_refl). inv Heq3; auto.
-      - exfalso. simpl_Exists.
-        eapply In_InMembers, fst_InMembers in Hin. rewrite Hfst in Hin.
-        eapply fst_InMembers, InMembers_In in Hin as (?&Hin).
-        unshelve simpl_Forall; eauto.
-      - exfalso. simpl_Exists.
-        eapply In_InMembers, fst_InMembers in Hin. rewrite <-Hfst in Hin.
-        eapply fst_InMembers, InMembers_In in Hin as (?&Hin).
-        unshelve simpl_Forall; eauto.
-      - econstructor; eauto.
-        + specialize (Heq3 _ _ eq_refl eq_refl). inv Heq3; auto.
-        + eapply IHn. 6,7:eauto. 1-5:intros; eauto.
-          erewrite 2 map_map, map_ext with (l:=xss1), map_ext with (l:=xss2); eauto; intros (?&?); auto.
-          erewrite fst_NoDupMembers, map_map, map_ext, <-fst_NoDupMembers; eauto; intros (?&?); auto.
-          (rewrite Forall2_map_1, Forall2_map_2; eapply Forall2_impl_In; [|eauto];
-           intros (?&?) (?&?) _ _ Heq; inv Heq; simpl in *; subst; auto).
-          inv H. inv H0.
-          specialize (Heq3 _ _ eq_refl eq_refl). inv Heq3; eauto.
-    Qed.
-
-    Lemma bools_of_detn : forall n xs1 xs2 bs1 bs2,
-        EqStN n xs1 xs2 ->
-        bools_of xs1 bs1 ->
-        bools_of xs2 bs2 ->
-        EqStN n bs1 bs2.
-    Proof.
-      induction n; intros * Heq Hbools1 Hbools2;
-        inv Heq; inv Hbools1; inv Hbools2; eauto.
-    Qed.
-
-    Lemma disj_str_detn : forall n xss1 xss2 bs1 bs2,
-        Forall2 (EqStN n) xss1 xss2 ->
-        bs1 ≡ disj_str xss1 ->
-        bs2 ≡ disj_str xss2 ->
-        EqStN n bs1 bs2.
-    Proof.
-      intros * Heq Hdisj1 Hdisj2.
-      eapply EqStN_spec. intros * Hlt.
-      eapply eqst_ntheq in Hdisj1. eapply eqst_ntheq in Hdisj2.
-      rewrite Hdisj1, Hdisj2.
-      repeat rewrite disj_str_spec.
-      clear - Heq Hlt.
-      induction Heq; simpl; auto.
-      rewrite IHHeq. f_equal; auto.
-      eapply EqStN_spec; eauto.
-    Qed.
-
-    Corollary bools_ofs_detn : forall n xss1 xss2 bs1 bs2,
-        Forall2 (EqStN n) xss1 xss2 ->
-        bools_ofs xss1 bs1 ->
-        bools_ofs xss2 bs2 ->
-        EqStN n bs1 bs2.
-    Proof.
-      intros * Heq (?&Hb1&Hdisj1) (?&Hb2&Hdisj2).
-      eapply disj_str_detn. 2,3:eauto.
-      clear - Heq Hb1 Hb2.
-      revert x x0 Hb1 Hb2.
-      induction Heq; intros; inv Hb1; inv Hb2; constructor; eauto.
-      eapply bools_of_detn; eauto.
-    Qed.
-
-    (* Fact det_exps_n' : forall n Hi1 Hi2 bs1 bs2 es ss1 ss2, *)
-    (*     Forall (fun e => forall ss1 ss2, *)
-    (*                 wt_exp G Γ e -> *)
-    (*                 sem_exp G Hi1 bs1 e ss1 -> *)
-    (*                 sem_exp G Hi2 bs2 e ss2 -> *)
-    (*                 Forall2 (EqStN n) ss1 ss2) es -> *)
-    (*     Forall (wt_exp G Γ) es-> *)
-    (*     Forall2 (sem_exp G Hi1 bs1) es ss1 -> *)
-    (*     Forall2 (sem_exp G Hi2 bs2) es ss2 -> *)
-    (*     Forall2 (EqStN n) (concat ss1) (concat ss2). *)
-    (* Proof. *)
-    (*   intros * Hf. revert ss1 ss2. *)
-    (*   induction Hf; intros * Hwt Hsem1 Hsem2; *)
-    (*     inv Hwt; inv Hsem1; inv Hsem2; simpl; auto. *)
-    (*   apply Forall2_app; eauto. *)
-    (* Qed. *)
-
-    (* Lemma Forall2Brs_det_exp_n' : forall n H1 H2 bs1 bs2 es ss1 ss2, *)
-    (*     Forall *)
-    (*       (fun es => *)
-    (*          Forall *)
-    (*            (fun e => *)
-    (*               forall ss1 ss2, *)
-    (*                 wt_exp G Γ e -> *)
-    (*                 sem_exp G H1 bs1 e ss1 -> sem_exp G H2 bs2 e ss2 -> Forall2 (EqStN n) ss1 ss2) *)
-    (*            (snd es)) es -> *)
-    (*     length ss1 = length ss2 -> *)
-    (*     Forall (fun es => Forall (wt_exp G Γ) (snd es)) es -> *)
-    (*     Forall2Brs (sem_exp G H1 bs1) es ss1 -> *)
-    (*     Forall2Brs (sem_exp G H2 bs2) es ss2 -> *)
-    (*     Forall2 (Forall2 (fun xs1 xs2 => EqStN n (snd xs1) (snd xs2))) ss1 ss2. *)
-    (* Proof. *)
-    (*   induction es; intros * Hf Hlen Hwt Hsem1 Hsem2; *)
-    (*     inv Hf; inv Hwt; inv Hsem1; inv Hsem2; simpl. *)
-    (*   - revert ss2 Hlen H0. *)
-    (*     induction H; intros * Hl Hf2; destruct ss2; simpl in *; try congruence; inv Hf2. *)
-    (*     1,2:constructor; eauto. *)
-    (*   - eapply IHes in H4. 3-5:eauto. clear IHes. *)
-    (*     2:{ eapply Forall3_length in H10 as (?&?). eapply Forall3_length in H14 as (?&?). *)
-    (*         congruence. *)
-    (*     } *)
-    (*     eapply det_exps_n' in H3; eauto. *)
-    (*     clear - H3 H4 H10 H14. revert vs2 vs3 H10 H14 H3 H4. *)
-    (*     generalize (concat vs0) (concat vs1); clear vs0 vs1. *)
-    (*     intros * Hf1. revert l ss2 vs3. *)
-    (*     induction Hf1; intros * Hf2 Heq1 Heq2; inv Heq1; inv Heq2; inv Hf2; constructor; eauto. *)
-    (* Qed. *)
-
-    Lemma denot_exps_nprod :
-      forall n env bs es,
-        Forall (fun e => forall_nprod (fun s => is_cons (nrem n s)) (denot_exp e env bs)) es ->
-        forall_nprod (fun s => is_cons (nrem n s)) (denot_exps es env bs).
-    Proof.
-      induction es; simpl in *; intros; auto; simpl_Forall.
-      setoid_rewrite denot_exps_eq; auto using forall_nprod_app.
-    Qed.
-
-    (* TODO: move *)
-    Lemma Forall_impl2 : forall {A} (P Q : A -> Prop) l,
-        Forall (fun x => P x -> Q x) l -> Forall P l -> Forall Q l.
-    Proof.
-      intros.
-      rewrite Forall_forall in *. firstorder.
-    Qed.
-
-    (** The clocking hypothesis could be replaced with a typing one.
-        The important point is that all the variables appearing in the expression
-        are in `env`.
-        I chose a clocking hypothesis because this lemma is used in the
-        clocked-semantics proof. *)
-    Lemma inf_exp_n : forall n env bs,
-        (forall x cx, HasCaus Γ x cx \/ HasLastCaus Γ x cx -> inf_var_inv n env cx) ->
-        is_cons (nrem n bs) ->
-        forall e,
-        wt_exp G Γ e ->
-        restr_exp e ->
-        forall_nprod (fun s => is_cons (nrem n s)) (denot_exp e env bs).
-    Proof.
-      intros * Hn Hb.
-      induction e using exp_ind2; intros * Hwt Hr; inv Hr; inv Hwt.
-      - (* const *)
-        rewrite denot_exp_eq.
-        apply is_consn_sconst; auto.
-      - (* var *)
-        rewrite denot_exp_eq.
-        inv H1.
-        eapply Hn; eauto. left.
-        all: econstructor; solve_In; eauto.
-      - (* unop *)
-        rewrite denot_exp_eq; simpl.
-        cases; try congruence; inv H4. (* typeof *)
-        assert (forall_nprod (fun s => is_cons (nrem n s)) (denot_exp e env0 bs)) as He by auto.
-        revert He.
-        generalize (denot_exp e env0 bs).
-        generalize (numstreams e).
-        intros ns t Ht.
-        cases; auto using is_consn_DS_const. (* numstreams *)
-        apply is_consn_sunop; auto.
-      - (* fby *)
-        rewrite denot_exp_eq; simpl.
-        unfold eq_rect_r, eq_rect.
-        cases.
-        apply forall_nprod_lift2; cases;
-          now eauto using is_consn_fby, denot_exps_nprod, Forall_impl2.
-        all: apply forall_nprod_k; intros; rewrite get_nth_const;
-          now auto using is_consn_DS_const.
-    Qed.
-
-    Corollary inf_exps_n : forall n env bs es,
-        (forall x cx, HasCaus Γ x cx \/ HasLastCaus Γ x cx -> inf_var_inv n env cx) ->
-        is_cons (nrem n bs) ->
-        Forall (wt_exp G Γ) es ->
-        Forall restr_exp es ->
-        forall_nprod (fun s => is_cons (nrem n s)) (denot_exps es env bs).
-    Proof.
-      intros * Hin Hb Hwt Hr.
-      induction es; simpl; auto; simpl_Forall.
-      setoid_rewrite denot_exps_eq; auto using forall_nprod_app, inf_exp_n.
-    Qed.
-
-    (* TODO: move *)
-    Lemma forall_nprod_impl :
-      forall (P Q : DS (sampl value) -> Prop),
-        (forall x, P x -> Q x) ->
-        forall {n} (np : nprod n),
-        forall_nprod P np ->
-        forall_nprod Q np.
-    Proof.
-      induction n as [|[]]; intros * Hf; auto.
-      - now simpl in *; auto.
-      - destruct Hf.
-        split; auto.
-        now apply IHn.
-    Qed.
-
-    Corollary inf_exp : forall env bs e,
-        wt_exp G Γ e ->
-        restr_exp e ->
-        forall_nprod (fun s => infinite s) (denot_exp e env bs).
-    Proof.
-      intros * Hwt Hr.
-      apply forall_nprod_impl with (1 := nrem_inf).
-      apply forall_nprod_k. intros k Hk n.
-      pose proof (inf_exp_n n) as Hn.
-      eapply forall_nprod_k' in Hn; eauto.
-      + intros * ???.
-        (* impossible, bien sûr *)
-    Abort.
-
-    (* Corollary det_exps : forall Hi bs es ss1 ss2, *)
-    (*     Forall (wt_exp G Γ) es -> *)
-    (*     Forall2 (sem_exp G Hi bs) es ss1 -> *)
-    (*     Forall2 (sem_exp G Hi bs) es ss2 -> *)
-    (*     EqSts (concat ss1) (concat ss2). *)
-    (* Proof. *)
-    (*   intros * Hwt Hs1 Hs2. *)
-    (*   eapply EqStN_EqSts. intros n. *)
-    (*   eapply det_exps_n; eauto. *)
-    (*   + intros * _ ???. *)
-    (*     split; intros; eapply EqStN_EqSt, sem_var_det; eauto. *)
-    (*   + reflexivity. *)
-    (* Qed. *)
-
-    (** We reason inductively on the length of streams.
-        Given that all the streams in the environnement are equal "up-to",
-        we need to proove that they are equal "up-to" n+1.
-        This can be established using causality, by following the causal order of the variables.
-        The interesting case is the fby operator, where the causality hypothesis doesn't tell us
-        anything about the expression on the right.
-        Fortunately, the following lemma indicates that we only need to know about equality "up-to" n
-        for the right-side stream of a fby, as the output only depends on its previous value.
-     *)
-
-    (* Lemma fby_det_Sn : forall n xs1 xs2 ys1 ys2 zs1 zs2, *)
-    (*     EqStN (S n) xs1 xs2 -> *)
-    (*     EqStN n ys1 ys2 -> *)
-    (*     fby xs1 ys1 zs1 -> *)
-    (*     fby xs2 ys2 zs2 -> *)
-    (*     EqStN (S n) zs1 zs2. *)
-    (* Proof. *)
-    (*   induction n; intros * Heq1 Heq2 Hfby1 Hfby2; inv Heq1; inv Heq2; *)
-    (*     inv Hfby1; inv Hfby2; constructor; auto. eauto. *)
-    (*   clear IHn. revert y xs0 xs1 xs3 xs2 rs rs0 H1 H2 H6 H7. *)
-    (*   induction n; intros * Heq1 Heq2 Hfby1 Hfby2; inv Heq1; inv Heq2; *)
-    (*     inv Hfby1; inv Hfby2; constructor; eauto. *)
-    (* Qed. *)
-
-    (* TODO: move *)
-    Lemma lift2_nth :
-      forall (f : forall A, DS (sampl A) -C-> DS (sampl A) -C-> DS (sampl A)),
-      forall {n} (np np' : nprod n) k,
-        k < n ->
-        get_nth (lift2 f np np') k = f _ (get_nth np k) (get_nth np' k).
-    Proof.
-      induction n as [|[]]; intros; auto; try lia.
-      - destruct k; simpl; auto; lia.
-      - destruct np, np'.
-        rewrite lift2_simpl.
-        destruct k; auto.
-        rewrite <- 3 get_nth_skip, <- IHn; auto with arith.
-    Qed.
-
-    Lemma inf_exp_S : forall n env bs,
-        (forall x cx, HasCaus Γ x cx \/ HasLastCaus Γ x cx -> inf_var_inv n env cx) ->
-        is_cons (nrem (S n) bs) ->
-        forall e k,
-          wt_exp G Γ e ->
-          restr_exp e ->
-          k < numstreams e ->
-          (forall x, Is_free_left Γ x k e -> inf_var_inv (S n) env x) ->
-          inf_exp_inv (S n) env bs e k.
-    Proof.
-      intros n env * Hn Hbs e k.
-      intros I J K L.
-      eapply exp_causal_ind
-        with (P_exp:=inf_exp_inv (S n) env bs); eauto with ltyping.
-      all: clear I J K L e k.
-      all: intros.
-      all: intros Hwt Hr; inv Hr; inv Hwt.
-      - (* const *)
-        rewrite denot_exp_eq.
-        now apply is_consn_sconst.
-      - (* var *)
-        rewrite denot_exp_eq.
-        now apply H0.
-      - (* unop *)
-        rewrite denot_exp_eq.
-        cases; try congruence; inv H5. (* typeof *)
-        assert (is_cons (nrem (S n) (get_nth (denot_exp e1 env bs) 0))) as He by auto.
-        revert He.
-        generalize (denot_exp e1 env bs).
-        generalize (numstreams e1).
-        intros ns t Ht.
-        cases.
-        2: apply is_consn_DS_const. (* pourquoi auto ne fonctionne pas ? *)
-        apply is_consn_sunop; auto.
-      - (* fby *)
-        rewrite denot_exp_eq; simpl.
-        unfold eq_rect_r, eq_rect.
-        cases.
-        2,3: rewrite get_nth_const; auto; apply (is_consn_DS_const _ (S n)).
-        rewrite lift2_nth; auto; cases.
-        apply is_consn_S_fby; auto using P_exps_inf_exp_inv.
-        apply forall_nprod_k'; auto using inf_exps_n, is_consn_S.
-    Qed.
-
-
-    Hypothesis Hnd : NoDup (map snd (idcaus_of_senv Γ)).
-
-    Lemma det_equation_S : forall n Hi1 Hi2 bs1 bs2 xs es k cx,
-        wt_equation G Γ (xs, es) ->
-        Sem.sem_equation G Hi1 bs1 (xs, es) ->
-        Sem.sem_equation G Hi2 bs2 (xs, es) ->
-        k < length xs ->
-        P_exps (det_exp_inv (S n) Hi1 Hi2 bs1 bs2) es k ->
-        HasCaus Γ (nth k xs xH) cx ->
-        det_var_inv (S n) Hi1 Hi2 cx.
-    Proof.
-      intros * (* Hn  *)(Hwt1&Hwt2) Hsem1 Hsem2 Hnum HSn Hin.
-      inv Hsem1. inv Hsem2.
-      eapply P_exps_det_exp_inv in HSn; eauto.
-      intros ???. split; intros Hin' Hv1 Hv2.
-      - eapply Forall2_forall2 in H5 as (Hl1&Heq1).
-        eapply Forall2_forall2 in H7 as (Hl2&Heq2).
-        eapply HasCaus_snd_det in Hin; eauto; subst.
-        eapply EqStN_morph. 3:eauto.
-        1,2:eapply sem_var_det; eauto.
-      - exfalso. eapply NoDup_HasCaus_HasLastCaus; eauto.
-    Qed.
-
-  End sem_equation_det.
-
-  Lemma det_var_inv_mask : forall Γ n rs1 rs2 Hi1 Hi2 x,
-      EqStN n rs1 rs2 ->
-      det_var_inv Γ n Hi1 Hi2 x ->
-      forall k, det_var_inv Γ n (mask_hist k rs1 Hi1) (mask_hist k rs2 Hi2) x.
+  Lemma HasCausRefl : forall Γ x, IsVar Γ x -> HasCaus Γ x x.
   Proof.
-    intros * Heq Hdet ????.
-    split; intros Hin Hv1 Hv2.
-    1,2:(eapply sem_var_mask_inv in Hv1 as (?&Hv1&Heq1);
-         eapply sem_var_mask_inv in Hv2 as (?&Hv2&Heq2);
-         rewrite Heq1, Heq2;
-         eapply EqStN_mask; eauto;
-         eapply Hdet in Hv2; eauto).
+    intros * Hv.
+    inv Hv.
+    apply InMembers_In in H as [e Hin].
+    econstructor; eauto.
+    erewrite HasCausInj; eauto using HasCaus.
   Qed.
 
-  Lemma det_var_inv_unmask : forall Γ n rs1 rs2 Hi1 Hi2 x,
-      EqStN n rs1 rs2 ->
-      (forall k, det_var_inv Γ n (mask_hist k rs1 Hi1) (mask_hist k rs2 Hi2) x) ->
-      det_var_inv Γ n Hi1 Hi2 x.
+  Lemma idcaus_map :
+    forall l : list (ident * (type * clock * ident)),
+      map snd (idcaus l) = map fst l.
   Proof.
-    intros * Heq Hdet ???.
-    split; intros Hin Hv1 Hv2; eapply EqStN_unmask; eauto;
-      intros k; [edestruct Hdet as (Hd&_)|edestruct Hdet as (_&Hd)];
-      eapply Hd; unfold mask_hist; eauto using sem_var_mask.
+    intros.
+    rewrite <- map_fst_senv_of_inout.
+    unfold idcaus, senv_of_inout.
+    rewrite 2 map_map.
+    apply map_ext_in_iff.
+    intros (x & (ty&c) &cx) Hin; simpl.
+    apply symmetry, HasCausInj with (Γ := senv_of_inout l).
+    econstructor.
+    apply in_map_iff; esplit; split; eauto.
+    all: eauto.
   Qed.
 
-  Lemma det_var_inv_filter : forall Γ n sc1 sc2 Hi1 Hi2 Hi1' Hi2' x,
-      EqStN n sc1 sc2 ->
-      det_var_inv Γ n Hi1 Hi2 x ->
-      forall c, filter_hist c sc1 Hi1 Hi1' ->
-           filter_hist c sc2 Hi2 Hi2' ->
-           det_var_inv Γ n Hi1' Hi2' x.
+  (** Invariants pour l'induction causale *)
+  Definition P_var (n : nat) (env : DS_prod SI) (x : ident) : Prop :=
+    is_cons (nrem n (PROJ _ x env)).
+
+  Definition P_vars (n : nat) (env : DS_prod SI) (cxs : list ident) : Prop :=
+    Forall (P_var n env) cxs.
+
+  Definition P_exp (n : nat) ins envI bs env (e : exp) (k : nat) : Prop :=
+    let ss := denot_exp ins e envI bs env in
+    is_cons (nrem n (get_nth ss k)).
+
+  Lemma P_vars_In :
+    forall n env xs x,
+      P_vars n env xs ->
+      In x xs ->
+      P_var n env x.
   Proof.
-    intros * Heq Hdet * (Hf11&Hf12) (Hf21&Hf22).
-    split; intros Hin Hv1 Hv2.
-    - eapply sem_var_filter_inv in Hv1 as (?&Hv1&Heq1); eauto.
-      eapply sem_var_filter_inv in Hv2 as (?&Hv2&Heq2); eauto.
-      apply filter_ffilter in Heq1. apply filter_ffilter in Heq2. rewrite Heq1, Heq2.
-      eapply EqStN_ffilter; eauto.
-      eapply Hdet in Hv2; eauto.
-    - rewrite Hf12 in Hv1. rewrite Hf22 in Hv2.
-      apply sem_var_ffilter_inv in Hv1 as (?&Hv1&Heq1).
-      apply sem_var_ffilter_inv in Hv2 as (?&Hv2&Heq2).
-      rewrite Heq1, Heq2.
-      eapply EqStN_ffilter; eauto.
-      eapply Hdet in Hv2; eauto.
+    unfold P_vars.
+    setoid_rewrite Forall_forall.
+    auto.
   Qed.
 
-  Lemma det_var_inv_unfilter : forall Γ tn n sc1 sc2 Hi1 Hi2 x,
-      snd tn > 0 ->
-      wt_stream sc1 (Tenum tn) ->
-      wt_stream sc2 (Tenum tn) ->
-      EqStN n sc1 sc2 ->
-      (forall c, In c (seq 0 (snd tn)) ->
-            exists Hi1' Hi2',
-              (forall y, HasCaus Γ y x -> Env.In y (fst Hi1') /\ Env.In y (fst Hi2'))
-              /\ filter_hist c sc1 Hi1 Hi1'
-              /\ filter_hist c sc2 Hi2 Hi2'
-              /\ det_var_inv Γ n Hi1' Hi2' x) ->
-      (forall y, ~HasLastCaus Γ y x) ->
-      det_var_inv Γ n Hi1 Hi2 x.
+  Lemma P_var_S :
+    forall n env x,
+      P_var (S n) env x ->
+      P_var n env x.
   Proof.
-    intros * Hn Hwt1 Hwt2 Heq Hdet Hnin ???.
-    split; intros Hin Hv1 Hv2.
-    - eapply EqStN_unfilter. 4:eauto. 1-3:eauto.
-      intros k Hin'. edestruct Hdet as (Hi1'&Hi2'&(Hin1&Hin2)&(Hf1&_)&(Hf2&_)&Hdet'); eauto.
-      assert (exists vs1', sem_var (fst Hi1') x0 vs1') as (?&Hvar1) by (inv Hin1; do 2 econstructor; try reflexivity; eauto).
-      assert (exists vs1', sem_var (fst Hi2') x0 vs1') as (?&Hvar2) by (inv Hin2; do 2 econstructor; try reflexivity; eauto).
-      assert (Hvar1':=Hvar1). eapply sem_var_filter_inv in Hvar1' as (?&?&Hv1'); eauto.
-      assert (Hvar2':=Hvar2). eapply sem_var_filter_inv in Hvar2' as (?&?&Hv2'); eauto.
-      eapply sem_var_det in Hv1; eauto. eapply sem_var_det in Hv2; eauto.
-      do 2 esplit; eauto. rewrite Hv1, Hv2 in *. repeat split; eauto.
-      apply filter_ffilter in Hv1'. apply filter_ffilter in Hv2'.
-      edestruct Hdet' as (Hdet1&_). eapply Hdet1; eauto.
-    - exfalso. eapply Hnin; eauto.
+    unfold P_var.
+    eauto using is_consn_S.
   Qed.
 
-  Section sem_block_det.
-    Context {PSyn : block -> Prop}.
-    Context {prefs : PS.t}.
-    Variable (G: @global PSyn prefs).
-
-    Inductive sem_block_det (n : nat) (envS : list ident) : history -> history -> Stream bool -> Stream bool -> block -> Prop :=
-    | Sdetbeq : forall Hi1 Hi2 bs1 bs2 eq,
-        sem_equation G Hi1 bs1 eq ->
-        sem_equation G Hi2 bs2 eq ->
-        sem_block_det n envS Hi1 Hi2 bs1 bs2 (Beq eq)
-    | Sdetreset : forall Hi1 Hi2 bs1 bs2 blocks er sr1 sr2 r1 r2,
-        sem_exp G Hi1 bs1 er [sr1] ->
-        sem_exp G Hi2 bs2 er [sr2] ->
-        bools_of sr1 r1 ->
-        bools_of sr2 r2 ->
-        (forall k, Forall (sem_block_det n envS (mask_hist k r1 Hi1) (mask_hist k r2 Hi2) (maskb k r1 bs1) (maskb k r2 bs2)) blocks) ->
-        sem_block_det n envS Hi1 Hi2 bs1 bs2 (Breset blocks er)
-    | Sdetswitch : forall Hi1 Hi2 bs1 bs2 branches ec sc1 sc2,
-        sem_exp G Hi1 bs1 ec [sc1] ->
-        sem_exp G Hi2 bs2 ec [sc2] ->
-        wt_streams [sc1] (typeof ec) ->
-        wt_streams [sc2] (typeof ec) ->
-        Forall (fun blks => exists Hi1' Hi2',
-                    filter_hist (fst blks) sc1 Hi1 Hi1'
-                    /\ filter_hist (fst blks) sc2 Hi2 Hi2'
-                    /\ Forall (sem_block_det n envS
-                                            Hi1' Hi2'
-                                            (ffilterb (fst blks) sc1 bs1) (ffilterb (fst blks) sc2 bs2)) (snd blks)) branches ->
-        sem_block_det n envS Hi1 Hi2 bs1 bs2 (Bswitch ec branches)
-    | Sdetlocal : forall Hi1 Hi2 Hl1 Hl2 bs1 bs2 locs blocks Hi1' Hi2' Hl1' Hl2',
-        (forall x vs, sem_var Hi1' x vs -> ~InMembers x locs -> sem_var Hi1 x vs) ->
-        (forall x vs, sem_var Hi2' x vs -> ~InMembers x locs -> sem_var Hi2 x vs) ->
-
-        Env.refines (@EqSt _) Hl1 Hl1' ->
-        Env.refines (@EqSt _) Hl2 Hl2' ->
-
-        (forall x ty ck cx e0 clx,
-              In (x, (ty, ck, cx, Some (e0, clx))) locs ->
-              exists vs0 vs1 vs,
-                sem_exp G (Hi1', Hl1') bs1 e0 [vs0] /\ sem_var Hi1' x vs1 /\ fby vs0 vs1 vs /\ sem_var Hl1' x vs) ->
-        (forall x ty ck cx e0 clx,
-              In (x, (ty, ck, cx, Some (e0, clx))) locs ->
-              exists vs0 vs1 vs,
-                sem_exp G (Hi2', Hl2') bs2 e0 [vs0] /\ sem_var Hi2' x vs1 /\ fby vs0 vs1 vs /\ sem_var Hl2' x vs) ->
-
-        Forall (sem_block_det n envS (Hi1', Hl1') (Hi2', Hl2') bs1 bs2) blocks ->
-
-        Forall (det_var_inv (senv_of_locs locs)
-                            (pred n) (Hi1', Hl1') (Hi2', Hl2')) (map snd (idcaus_of_senv (senv_of_locs locs))) ->
-        Forall (fun x => In x envS -> det_var_inv (senv_of_locs locs) n (Hi1', Hl1') (Hi2', Hl2') x)
-               (map snd (idcaus_of_senv (senv_of_locs locs))) ->
-        sem_block_det n envS (Hi1, Hl1) (Hi2, Hl2) bs1 bs2 (Blocal locs blocks).
-
-    (* Initialize with two "simple" sems *)
-    Lemma sem_block_det_0 : forall envS blk Hi1 Hi2 bs1 bs2,
-        sem_block G Hi1 bs1 blk ->
-        sem_block G Hi2 bs2 blk ->
-        sem_block_det 0 envS Hi1 Hi2 bs1 bs2 blk.
-    Proof.
-      induction blk using block_ind2; intros * Hsem1 Hsem2;
-        inv Hsem1; inv Hsem2.
-      - (* equation *)
-        constructor; auto.
-      - (* reset *)
-        econstructor; eauto.
-        intros k. specialize (H7 k). specialize (H10 k).
-        rewrite Forall_forall in *; eauto.
-      - (* switch *)
-        econstructor; eauto. simpl_Forall.
-        do 2 esplit. split; [|split]; eauto.
-        simpl_Forall; eauto.
-      - (* locals *)
-        econstructor; eauto.
-        + rewrite Forall_forall in *; eauto.
-        + simpl_Forall. intros ???. split; intros; auto with coindstreams.
-        + simpl_Forall. intros ???. split; intros; auto with coindstreams.
-    Qed.
-
-    (* Go from n to n + 1 :) *)
-    Lemma sem_block_det_S : forall n envS blk Hi1 Hi2 bs1 bs2,
-        incl (map snd (idcaus_of_locals blk)) envS ->
-        sem_block_det n envS Hi1 Hi2 bs1 bs2 blk ->
-        sem_block_det (S n) [] Hi1 Hi2 bs1 bs2 blk.
-    Proof.
-      induction blk using block_ind2; intros * Hincl Hsem; inv Hsem; simpl in *.
-      - (* equation *)
-        constructor; eauto.
-      - (* reset *)
-        econstructor; eauto.
-        intros k. specialize (H10 k).
-        rewrite Forall_forall in *; intros; eauto.
-        eapply H; eauto. etransitivity. 2:eapply Hincl.
-        intros ??. solve_In.
-      - (* switch *)
-        econstructor; eauto. simpl_Forall.
-        do 2 esplit. split; [|split]; eauto.
-        simpl_Forall. eapply H; eauto.
-        etransitivity. 2:eapply Hincl.
-        intros ??. simpl_In. solve_In.
-      - (* locals *)
-        econstructor; eauto. 1-3:simpl_Forall.
-        + eapply H; eauto.
-          etransitivity. 2:eapply Hincl.
-          intros ??; simpl_In. eapply idcaus_of_locals_In_local1 in Hin; eauto. solve_In.
-        + eapply H14, Hincl.
-          eapply idcaus_of_locals_In_local2 in H0; eauto. solve_In.
-        + now exfalso.
-    Qed.
-
-    Fact sem_block_det_sem_block1 : forall n envS blk Hi1 Hi2 bs1 bs2,
-        sem_block_det n envS Hi1 Hi2 bs1 bs2 blk ->
-        sem_block G Hi1 bs1 blk.
-    Proof.
-      induction blk using block_ind2; intros * Hsem; inv Hsem.
-      - (* equation *)
-        constructor; auto.
-      - (* reset *)
-        econstructor; eauto.
-        intros k. specialize (H10 k). simpl_Forall; eauto.
-      - (* switch *)
-        econstructor; eauto.
-        simpl_Forall. do 2 esplit; eauto. simpl_Forall; eauto.
-      - (* locals *)
-        econstructor; eauto. simpl_Forall; eauto.
-    Qed.
-
-    Fact sem_block_det_sem_block2 : forall n envS blk Hi1 Hi2 bs1 bs2,
-        sem_block_det n envS Hi1 Hi2 bs1 bs2 blk ->
-        sem_block G Hi2 bs2 blk.
-    Proof.
-      induction blk using block_ind2; intros * Hsem; inv Hsem.
-      - (* equation *)
-        constructor; auto.
-      - (* reset *)
-        econstructor; eauto.
-        intros k. specialize (H10 k). simpl_Forall; eauto.
-      - (* switch *)
-        econstructor; eauto.
-        simpl_Forall. do 2 esplit; eauto. simpl_Forall; eauto.
-      - (* locals *)
-        econstructor; eauto. simpl_Forall; eauto.
-    Qed.
-
-    Hint Resolve sem_block_det_sem_block1 sem_block_det_sem_block2 : ldet.
-
-    Lemma det_var_inv_incl : forall Γ Γ' n Hi1 Hi2 x,
-        incl Γ Γ' ->
-        det_var_inv Γ' n Hi1 Hi2 x ->
-        det_var_inv Γ n Hi1 Hi2 x.
-    Proof.
-      intros * Hincl1 Hdet ???.
-      split; intros Hin Hv1 Hv2; eauto.
-      1,2:eapply Hdet in Hv2; eauto with senv.
-    Qed.
-
-    Import Permutation.
-
-    Lemma sem_block_det_Perm : forall n xs ys blk Hi1 Hi2 bs1 bs2,
-        Permutation xs ys ->
-        sem_block_det n xs Hi1 Hi2 bs1 bs2 blk ->
-        sem_block_det n ys Hi1 Hi2 bs1 bs2 blk.
-    Proof.
-      induction blk using block_ind2; intros * Hperm Hsem;
-        inv Hsem.
-      - (* equation *)
-        constructor; auto.
-      - (* reset *)
-        econstructor; eauto.
-        intros k. specialize (H10 k). simpl_Forall; eauto.
-      - (* switch *)
-        econstructor; eauto. simpl_Forall.
-        do 2 esplit. split; [|split]; eauto.
-        simpl_Forall; eauto.
-      - (* local *)
-        econstructor; eauto.
-        1:simpl_Forall; eauto.
-        setoid_rewrite <-Hperm; auto.
-    Qed.
-
-    Fact det_var_inv_local :
-      forall Γ (locs : list (ident * (type * clock * ident * option (exp * ident)))) Hi1 Hi2 Hl1 Hl2 Hi1' Hi2' Hl1' Hl2' n cx,
-        (forall x : ident, InMembers x locs -> ~ In x (map fst Γ)) ->
-        (forall x, IsLast Γ x -> Env.In x Hl1) ->
-        (forall x, IsLast Γ x -> Env.In x Hl2) ->
-        (forall x vs, sem_var Hi1' x vs -> ~ InMembers x locs -> sem_var Hi1 x vs) ->
-        (forall x vs, sem_var Hi2' x vs -> ~ InMembers x locs -> sem_var Hi2 x vs) ->
-        Env.refines (@EqSt _) Hl1 Hl1' ->
-        Env.refines (@EqSt _) Hl2 Hl2' ->
-        (forall x, HasCaus Γ x cx \/ HasLastCaus Γ x cx -> det_var_inv Γ n (Hi1, Hl1) (Hi2, Hl2) cx) ->
-        (forall x, HasCaus (senv_of_locs locs) x cx \/ HasLastCaus (senv_of_locs locs) x cx ->
-              det_var_inv (senv_of_locs locs) n (Hi1', Hl1') (Hi2', Hl2') cx) ->
-        det_var_inv (Γ ++ senv_of_locs locs) n (Hi1', Hl1') (Hi2', Hl2') cx.
-    Proof.
-      intros * Hnd Hdoml1 Hdoml2 Href1 Href2 Hrefl1 Hrefl2 Hsc1 Hsc2.
-      split; intros Hin Hv1 Hv2; inv Hin; rewrite in_app_iff in H; destruct H as [Hin|Hin]; simpl in *.
-      - edestruct Hsc1 as (Hinv&_); [|eapply Hinv]; eauto with senv.
-        + eapply Href1; eauto. intros Hnin.
-          eapply Hnd; eauto. solve_In.
-        + eapply Href2; eauto. intros Hnin.
-          eapply Hnd; eauto. solve_In.
-      - edestruct Hsc2 as (Hinv&_); [|eapply Hinv]; eauto with senv.
-      - edestruct Hsc1 as (_&Hinv); [|eapply Hinv]; eauto with senv.
-        1,2:eapply sem_var_refines'; eauto with senv.
-        + eapply Hdoml1. econstructor; eauto. congruence.
-        + eapply Hdoml2. econstructor; eauto. congruence.
-      - edestruct Hsc2 as (_&Hinv); [|eapply Hinv]; eauto with senv.
-    Qed.
-
-    Lemma det_block_S : forall n envS blk Γ xs Hi1 Hi2 bs1 bs2 y cy,
-        det_nodes G ->
-        NoDup (map snd (idcaus_of_senv Γ ++ idcaus_of_locals blk)) ->
-        NoDupLocals (map fst Γ) blk ->
-        VarsDefined blk xs ->
-        incl xs (map fst Γ) ->
-        (forall x, IsLast Γ x -> Env.In x (snd Hi1)) ->
-        (forall x, IsLast Γ x -> Env.In x (snd Hi2)) ->
-        (forall x cx, HasCaus Γ x cx \/ HasLastCaus Γ x cx -> det_var_inv Γ n Hi1 Hi2 cx) ->
-        wt_block G Γ blk ->
-        sem_block_det (S n) envS Hi1 Hi2 bs1 bs2 blk ->
-        EqStN (S n) bs1 bs2 ->
-        In y xs ->
-        HasCaus Γ y cy ->
-        (forall x cx, HasCaus Γ x cx \/ HasLastCaus Γ x cx ->
-                 depends_on Γ cy cx blk -> det_var_inv Γ (S n) Hi1 Hi2 cx) ->
-        (forall cx, In cx (map snd (idcaus_of_locals blk)) ->
-               depends_on Γ cy cx blk -> In cx envS) ->
-        det_var_inv Γ (S n) Hi1 Hi2 cy.
-    Proof.
-      induction blk as [(xs&es)| | |] using block_ind2;
-        intros * HdetG Hnd Hnd2 Hvars Hincl Hdom1 Hdom2 Hn Hwt Hsem Hbs Hinxs Hinenv HSn HenvS;
-        inv Hnd2; inv Hvars; inv Hwt; inv Hsem; simpl in *.
-      - (* equation *)
-        eapply In_nth in Hinxs as (?&Hlen&Hnth). instantiate (1:=xH) in Hnth.
-        rewrite app_nil_r in Hnd.
-        eapply det_equation_S; eauto.
-        + eapply Pexp_Pexps.
-          * simpl_Forall.
-            eapply det_exp_S; eauto.
-          * intros ? IsF. assert (IsF':=IsF). eapply Is_free_left_list_In_snd in IsF as (?&?).
-            eapply HSn; eauto.
-            rewrite <-Hnth in *. econstructor; eauto using nth_error_nth'.
-          * destruct H1 as (_&Hf2). apply Forall2_length in Hf2.
-            rewrite <-length_typesof_annots. congruence.
-        + now rewrite Hnth.
-
-      - (* reset *)
-        eapply in_concat in Hinxs as (?&Hin1&Hin2). inv_VarsDefined. simpl_Forall.
-        assert (EqStN (S n) r1 r2) as Hrs.
-        { eapply bools_of_detn. 2,3:eauto.
-          eapply det_exp_S with (k:=0) (n:=n) in H5; eauto.
-          - eapply H5 in H8; simpl in H8; eauto.
-          - rewrite <-length_typeof_numstreams, H7; simpl. lia.
-          - intros ? IsF. assert (IsF':=IsF). eapply Is_free_left_In_snd in IsF as (?&?).
-            eapply HSn, DepOnReset2; eauto. solve_Exists.
-            left. eapply In_Is_defined_in with (Γ:=Γ); eauto using in_or_app.
-            etransitivity; eauto using incl_concat.
-        }
-        eapply det_var_inv_unmask; eauto.
-        intros k. specialize (H15 k). simpl_Forall.
-        eapply H with (bs1:=maskb k r1 bs1) (bs2:=maskb k r2 bs2); eauto.
-        + clear - Hinblks Hnd.
-          eapply NoDup_locals_inv; eauto.
-        + etransitivity; eauto using incl_concat.
-        + setoid_rewrite Env.Props.P.F.map_in_iff; eauto.
-        + setoid_rewrite Env.Props.P.F.map_in_iff; eauto.
-        + intros. eapply det_var_inv_mask; eauto using EqStN_weaken.
-        + eapply EqStN_mask; eauto.
-        + intros * Hin' Hdep. eapply det_var_inv_mask; eauto.
-          eapply HSn; eauto. constructor. solve_Exists.
-        + intros * Hin' Hdep. eapply HenvS; eauto.
-          2:constructor; solve_Exists. solve_In.
-
-      - (* switch *)
-        assert (Is_defined_in Γ cy (Bswitch ec branches)) as Hdef.
-        { eapply In_Is_defined_in with (Γ:=Γ); eauto using incl_refl, in_or_app.
-          econstructor; eauto. }
-        eapply det_exp_S with (k:=0) (n:=n) in H9; eauto. specialize (H9 H12); simpl in H9.
-        2:{ rewrite <-length_typeof_numstreams, H6; auto. }
-        2:{ intros ? IsF. assert (IsF':=IsF). eapply Is_free_left_In_snd in IsF as (?&?).
-            eapply HSn, DepOnSwitch2; eauto.
-            inv Hdef. solve_Exists. }
-        repeat (take (wt_streams [_] (typeof ec)) and rewrite H6 in it; apply Forall2_singl in it).
-        eapply det_var_inv_unfilter. 4:eauto. all:eauto.
-        1:{ destruct tn as (?&[]); simpl in *; try lia.
-            apply Permutation_sym, Permutation_nil, map_eq_nil in H8; congruence. }
-        2:{ intros * Hnin. eapply NoDup_HasCaus_HasLastCaus; eauto. solve_NoDup_app. }
-        intros ? Hseq.
-        assert (exists blks, In (c, blks) branches) as (blks&Hinbrs).
-        { rewrite <-H8 in Hseq. simpl_In; eauto. }
-        repeat (take (Forall _ branches) and eapply Forall_forall in it; eauto).
-        destruct it4 as (?&Hvars&Hperm).
-        rewrite <-Hperm in Hinxs. apply in_concat in Hinxs as (?&Hin1&Hin2).
-        eapply Forall2_ignore1, Forall_forall in Hvars as (?&Hinblk&?); eauto; simpl in *.
-        simpl_Forall. do 2 esplit. split; [|split; [|split]]; eauto.
-        1:{ intros ? Hcaus.
-            eapply HasCaus_snd_det in Hinenv; eauto; subst. 2:simpl_app; eauto using NoDup_app_l.
-            split; eapply sem_block_defined; eauto using sem_block_det_sem_block1, sem_block_det_sem_block2.
-            1,2:(eapply VarsDefined_Is_defined in H; eauto;
-                 eapply NoDupLocals_incl; [|eauto]; etransitivity; eauto;
-                 rewrite <-Hperm; eauto using incl_concat).
-        }
-        eapply it; eauto.
-        + clear - Hinbrs Hinblk Hnd.
-          eapply NoDup_locals_inv, NoDup_locals_inv2; eauto. auto.
-        + etransitivity; [|eauto]. rewrite <-Hperm. eapply incl_concat; eauto.
-        + destruct H0 as (?&Heq). setoid_rewrite Heq. setoid_rewrite Env.Props.P.F.map_in_iff; eauto.
-        + destruct H1 as (?&Heq). setoid_rewrite Heq. setoid_rewrite Env.Props.P.F.map_in_iff; eauto.
-        + intros * Hin. eapply det_var_inv_filter; eauto using EqStN_weaken.
-        + eapply EqStN_ffilter; eauto.
-        + intros * Hin Hdep. eapply det_var_inv_filter; eauto.
-          eapply HSn; eauto.
-          constructor. solve_Exists.
-        + intros * Hin Hdep. eapply HenvS; eauto.
-          * solve_In.
-          * constructor. solve_Exists.
-
-      - (* locals *)
-        assert (In y (concat xs0)) as Hinxs0 by (rewrite <-H7; auto with datatypes).
-        eapply in_concat in Hinxs0 as (?&Hin1&Hin2).
-        eapply Forall2_ignore1, Forall_forall in H3 as (?&Hinblk&Hvars); eauto.
-        eapply Forall_forall in H; eauto.
-        assert (det_var_inv (Γ ++ senv_of_locs locs)
-                            (S n) (Hi1', Hl1') (Hi2', Hl2') cy) as Hdet'.
-        { eapply H; eauto.
-          - clear - Hinblk Hnd.
-            eapply NoDup_locals_inv; eauto. rewrite idcaus_of_senv_app.
-            simpl_app. auto.
-          - simpl_Forall. now rewrite map_app, map_fst_senv_of_locs.
-          - rewrite map_app, map_fst_senv_of_locs.
-            etransitivity; eauto using incl_concat.
-            rewrite <-H7, Permutation_app_comm.
-            apply incl_app; [apply incl_appl|apply incl_appr]; eauto using incl_refl.
-          - intros * Hin. inv Hin.
-            apply in_app_iff in H0 as [|]; simpl_In; subst.
-            + eapply Env.In_refines; eauto with senv.
-            + destruct o as [(?&?)|]; simpl in *; try congruence.
-              edestruct H15 as (?&?&?&?&?&?&?); eauto using sem_var_In.
-          - intros * Hin. inv Hin.
-            apply in_app_iff in H0 as [|]; simpl_In; subst.
-            + eapply Env.In_refines; eauto with senv.
-            + destruct o as [(?&?)|]; simpl in *; try congruence.
-              edestruct H16 as (?&?&?&?&?&?&?); eauto using sem_var_In.
-          - intros * _. eapply det_var_inv_local with (Hl1:=Hl1); eauto.
-            intros ? Hin. eapply Forall_forall in H22; eauto.
-            apply idcaus_of_senv_In in Hin. solve_In.
-          - simpl_Forall; auto.
-          - simpl_Forall; auto.
-          - apply HasCaus_app; auto.
-          - intros * _ Hdep. eapply det_var_inv_local with (Hl1:=Hl1); eauto.
-            + intros. eapply HSn; eauto.
-              econstructor; eauto. solve_Exists.
-            + intros * Hin.
-              assert (In cx (map snd (idcaus_of_senv (senv_of_locs locs)))) as Hin'.
-              { apply idcaus_of_senv_In in Hin. solve_In. }
-              eapply Forall_forall in H23; eauto. eapply H23.
-              eapply HenvS.
-              * simpl_In. eapply idcaus_of_locals_In_local2 in Hin0; eauto. solve_In.
-              * econstructor; eauto. solve_Exists.
-          - intros * Hin Hdep. apply HenvS.
-            + simpl_In. eapply idcaus_of_locals_In_local1 in Hin0; eauto. solve_In.
-            + econstructor; eauto. solve_Exists.
-        }
-        intros ???. split; intros Hin3 Hv1 Hv2.
-        + eapply HasCaus_snd_det in Hinenv; eauto; subst. 2:solve_NoDup_app.
-          assert (~InMembers y locs) as Hnin.
-          { intros ?. eapply H5; eauto. }
-          assert (NoDupLocals x x0).
-          { rewrite Forall_forall in *. eapply NoDupLocals_incl; eauto.
-            etransitivity; eauto using incl_concat.
-            rewrite <-H7, Permutation_app_comm.
-            apply incl_app; [apply incl_appl; auto|apply incl_appr, incl_refl].
-          }
-          edestruct Hdet' as (Hd1&_). eapply Hd1; [eapply HasCaus_app| |]; eauto.
-          1,2:(eapply sem_var_refines_inv; [| | |eauto]; intros; eauto).
-          1,2:rewrite Forall_forall in *; eapply sem_block_dom_lb; eauto with ldet.
-        + exfalso. eapply NoDup_HasCaus_HasLastCaus; eauto. solve_NoDup_app.
-    Qed.
-
-    Lemma sem_block_det_cons_nIn : forall n envS x blk Hi1 Hi2 bs1 bs2,
-        ~In x (map snd (idcaus_of_locals blk)) ->
-        sem_block_det n envS Hi1 Hi2 bs1 bs2 blk ->
-        sem_block_det n (x::envS) Hi1 Hi2 bs1 bs2 blk.
-    Proof.
-      induction blk using block_ind2; intros * Hnin Hsem;
-        simpl in *; inv Hsem.
-      - (* equation *)
-        constructor; auto.
-      - (* reset *)
-        econstructor; eauto.
-        intros k. specialize (H10 k).
-        rewrite Forall_forall in *; intros. eapply H; eauto.
-        contradict Hnin. solve_In.
-      - (* switch *)
-        econstructor; eauto. simpl_Forall.
-        do 2 esplit; split; [|split]; eauto. simpl_Forall.
-        eapply H; eauto.
-        contradict Hnin. solve_In.
-      - (* locals *)
-        econstructor; eauto.
-        + rewrite Forall_forall in *; intros. eapply H; eauto.
-          contradict Hnin.
-          simpl_In. eapply idcaus_of_locals_In_local1 in Hin; eauto. solve_In.
-        + eapply Forall_impl_In; [|eapply H14]; intros * Hin1 Hloc Hin2.
-          inv Hin2; eauto.
-          exfalso. eapply Hnin. simpl_In. eapply idcaus_of_locals_In_local2 in Hin; eauto. solve_In.
-    Qed.
-
-    Lemma sem_block_det_cons_In : forall n envS blk Γ xs Hi1 Hi2 bs1 bs2 y cy,
-        det_nodes G ->
-        NoDup (map snd (idcaus_of_senv Γ ++ idcaus_of_locals blk)) ->
-        NoDupLocals (map fst Γ) blk ->
-        VarsDefined blk xs ->
-        incl xs (map fst Γ) ->
-        (forall x, IsLast Γ x -> Env.In x (snd Hi1)) ->
-        (forall x, IsLast Γ x -> Env.In x (snd Hi2)) ->
-        (forall x cx, HasCaus Γ x cx \/ HasLastCaus Γ x cx -> det_var_inv Γ n Hi1 Hi2 cx) ->
-        wt_block G Γ blk ->
-        sem_block_det (S n) envS Hi1 Hi2 bs1 bs2 blk ->
-        EqStN (S n) bs1 bs2 ->
-        In (y, cy) (idcaus_of_locals blk) ->
-        (forall x cx, HasCaus Γ x cx \/ HasLastCaus Γ x cx ->
-                 depends_on Γ cy cx blk -> det_var_inv Γ (S n) Hi1 Hi2 cx) ->
-        (forall cx, In cx (map snd (idcaus_of_locals blk)) ->
-               depends_on Γ cy cx blk -> In cx envS) ->
-        sem_block_det (S n) (cy::envS) Hi1 Hi2 bs1 bs2 blk.
-    Proof.
-      induction blk as [(xs&es)| | |] using block_ind2;
-        intros * HdetG Hnd Hnd2 Hvars Hincl Hdom1 Hdom2 Hn Hwt Hsem Hbs Hinenv HSn HenvS;
-        inv Hnd2; inv Hvars; inv Hwt; inv Hsem; simpl in *.
-      - (* equation *)
-        inv Hinenv.
-
-      - (* reset *)
-        econstructor; eauto. intros k. specialize (H15 k).
-        eapply Forall2_ignore2 in H4.
-        rewrite Forall_forall in *; intros * Hinblk.
-        destruct (in_dec ident_eq_dec cy (map snd (idcaus_of_locals x))).
-        2:eapply sem_block_det_cons_nIn; eauto.
-        edestruct H4 as (?&Hinvars&Hvars'); eauto.
-        assert (EqStN (S n) r1 r2) as Hrs.
-        { eapply bools_of_detn. 2,3:eauto.
-          eapply det_exp_S with (k:=0) (n:=n) in H5; eauto.
-          - eapply H5 in H8; eauto.
-          - rewrite <-length_typeof_numstreams, H7; simpl; lia.
-          - intros ? IsF. assert (IsF':=IsF). eapply Is_free_left_In_snd in IsF as (?&?).
-            eapply HSn, DepOnReset2; eauto. solve_Exists.
-            eapply idcaus_of_locals_def_last; eauto.
-            eapply NoDupLocals_incl; eauto. etransitivity; eauto using incl_concat.
-        }
-        { simpl_In.
-          eapply H with (Γ:=Γ); eauto; try solve_In.
-          - clear - Hinblk Hnd.
-            eapply NoDup_locals_inv; eauto.
-          - etransitivity; eauto using incl_concat.
-          - setoid_rewrite Env.Props.P.F.map_in_iff; eauto.
-          - setoid_rewrite Env.Props.P.F.map_in_iff; eauto.
-          - intros * ?.
-            eapply det_var_inv_mask; eauto using EqStN_weaken.
-          - eapply EqStN_mask; eauto.
-          - intros * Hin' Hdep.
-            eapply det_var_inv_mask; eauto. eapply HSn; eauto.
-            constructor. solve_Exists.
-          - intros * Hin' Hdep. eapply HenvS; eauto. solve_In.
-            constructor; solve_Exists.
-        }
-
-      - (* switch *)
-        econstructor; eauto. simpl_Forall.
-        do 2 esplit. split; [|split]; eauto.
-        simpl_Forall. inv_VarsDefined.
-        destruct (in_dec ident_eq_dec cy (map snd (idcaus_of_locals x0))).
-        2:eapply sem_block_det_cons_nIn; eauto. simpl_In.
-        eapply det_exp_S with (k:=0) (n:=n) in H9; eauto. specialize (H9 H12); simpl in H9.
-        2:{ rewrite <-length_typeof_numstreams, H6; auto. }
-        2:{ intros ? IsF. assert (IsF':=IsF). eapply Is_free_left_In_snd in IsF as (?&?).
-            eapply HSn, DepOnSwitch2; eauto. solve_Exists.
-            eapply idcaus_of_locals_def_last; eauto. 2:solve_In.
-            eapply NoDupLocals_incl; eauto. etransitivity; eauto.
-            take (Permutation _ _) and rewrite <-it; eauto using incl_concat.
-        }
-        repeat (take (wt_streams [_] (typeof ec)) and rewrite H6 in it; apply Forall2_singl in it).
-        eapply H; eauto.
-        + clear - H0 H17 Hnd.
-          eapply NoDup_locals_inv, NoDup_locals_inv2; eauto. auto.
-        + etransitivity; [|eauto]. take (Permutation _ _) and rewrite <-it. eapply incl_concat; eauto.
-        + destruct H1 as (?&Heq). setoid_rewrite Heq. setoid_rewrite Env.Props.P.F.map_in_iff; eauto.
-        + destruct H14 as (?&Heq). setoid_rewrite Heq. setoid_rewrite Env.Props.P.F.map_in_iff; eauto.
-        + intros * ??. eapply det_var_inv_filter; eauto using EqStN_weaken.
-        + eapply EqStN_ffilter; eauto.
-        + intros * ? Hdep. eapply det_var_inv_filter; eauto.
-          eapply HSn; eauto.
-          constructor. solve_Exists.
-        + intros ? Hin' Hdep. eapply HenvS; eauto. solve_In.
-          constructor. solve_Exists.
-
-      - (* locals *)
-        unfold idcaus_of_locals, idcaus_of_senv in Hinenv; simpl in *. rewrite 2 in_app_iff in Hinenv.
-        destruct Hinenv as [[Hinenv|Hinenv]|Hinenv].
-        + (* current locs *)
-          econstructor; eauto.
-          * rewrite Forall_forall in *; intros.
-            eapply sem_block_det_cons_nIn; eauto.
-            { intro Hin. clear - H0 Hinenv Hin Hnd. unfold idcaus_of_senv in Hnd.
-              simpl_app.
-              eapply NoDup_app_r, NoDup_app_r, NoDup_app_In with (x:=cy) in Hnd.
-              2:solve_In. clear Hinenv.
-              eapply Hnd. repeat rewrite in_app_iff in *. right. solve_In. }
-          * eapply Forall_impl_In; [|eauto]; intros ? Hin Hdet Hin'.
-            inv Hin'; eauto.
-            assert (In y (concat xs0)) as Hinvars.
-            { rewrite <-H7. apply in_or_app; left.
-              clear - Hinenv. solve_In. }
-            eapply in_concat in Hinvars as (xs'&?&Hinvars). inv_VarsDefined.
-            eapply det_var_inv_incl with (Γ':=Γ ++ senv_of_locs locs).
-            1:solve_incl_app.
-            { eapply det_block_S with (envS:=envS); eauto.
-              - clear - Hinblks Hnd.
-                eapply NoDup_locals_inv; eauto. rewrite idcaus_of_senv_app. simpl_app. auto.
-              - simpl_Forall. now rewrite map_app, map_fst_senv_of_locs.
-              - rewrite map_app, map_fst_senv_of_locs.
-                etransitivity; eauto using incl_concat.
-                rewrite <-H7, Permutation_app_comm.
-                apply incl_app; [apply incl_appl|apply incl_appr]; eauto using incl_refl.
-              - intros * Hin'. inv Hin'.
-                apply in_app_iff in H1 as [|]; simpl_In; subst.
-                + eapply Env.In_refines; eauto with senv.
-                + destruct o as [(?&?)|]; simpl in *; try congruence.
-                  edestruct H15 as (?&?&?&?&?&?&?); eauto using sem_var_In.
-              - intros * Hin'. inv Hin'.
-                apply in_app_iff in H1 as [|]; simpl_In; subst.
-                + eapply Env.In_refines; eauto with senv.
-                + destruct o as [(?&?)|]; simpl in *; try congruence.
-                  edestruct H16 as (?&?&?&?&?&?&?); eauto using sem_var_In.
-              - intros * _. eapply det_var_inv_local with (Hl1:=Hl1); eauto.
-                intros * Hin'. eapply Forall_forall in H22; eauto.
-                clear - Hin'. unfold idcaus_of_senv. simpl_app. rewrite in_app_iff; auto.
-                destruct Hin' as [Hin'|Hin']; inv Hin'; simpl_In; [left|right]; solve_In. auto.
-              - simpl_Forall; auto.
-              - simpl_Forall; auto.
-              - simpl_In. econstructor. apply in_or_app; right; solve_In. auto.
-              - intros * _ Hdep. eapply det_var_inv_local with (Hl1:=Hl1); eauto.
-                + intros. eapply HSn; eauto.
-                  econstructor; eauto. solve_Exists.
-                + intros * Hin'.
-                  assert (In cx (map snd (idcaus_of_senv (senv_of_locs locs)))) as Hin2.
-                  { apply idcaus_of_senv_In in Hin'. solve_In. }
-                  eapply Forall_forall with (x:=cx) in H23; eauto. eapply H23.
-                  eapply HenvS.
-                  * simpl_In. eapply idcaus_of_locals_In_local2 in Hin0; eauto. solve_In.
-                  * econstructor; eauto. solve_Exists.
-              - intros * Hin' Hdep. apply HenvS.
-                + simpl_In. eapply idcaus_of_locals_In_local1 in Hin0; eauto. solve_In.
-                + econstructor; eauto. solve_Exists.
-            }
-
-        + (* lasts *)
-          simpl_In; subst.
-          econstructor; eauto.
-          * rewrite Forall_forall in *; intros.
-            eapply sem_block_det_cons_nIn; eauto.
-            { intro Hin. clear - H0 Hin0 Hin Hnd. unfold idcaus_of_senv in Hnd.
-              simpl_app.
-              eapply NoDup_app_r, NoDup_app_r, NoDup_app_r, NoDup_app_In with (x:=i0) in Hnd.
-              2:solve_In; auto. clear Hin0.
-              eapply Hnd. repeat rewrite in_app_iff in *. solve_In. }
-          * apply Forall_forall; intros * Hin HinenvS. destruct HinenvS; subst; [|simpl_Forall; eauto].
-            simpl_In. unfold idcaus_of_senv, senv_of_locs in Hin1. apply in_app_iff in Hin1 as [|]; simpl_In; subst.
-            1:{ exfalso. clear - Hnd Hin1 Hin0. unfold idcaus_of_senv in Hnd. simpl_app.
-                eapply NoDup_app_r, NoDup_app_r, NoDup_app_In in Hnd. 2:solve_In.
-                eapply Hnd. repeat rewrite in_app_iff. left. clear Hin1. solve_In. auto.
-            }
-            edestruct H15 as (?&?&?&He1&Hv1&Hfby1&Hv'1); eauto.
-            edestruct H16 as (?&?&?&He2&Hv2&Hfby2&Hv'2); eauto.
-            split; intros * Hin' Hv Hv'.
-            1:{ exfalso. clear - Hnd Hin1 Hin'. inv Hin'. simpl_In.
-                unfold idcaus_of_senv in Hnd. simpl_app.
-                eapply NoDup_app_r, NoDup_app_r, NoDup_app_In in Hnd. 2:solve_In.
-                eapply Hnd. repeat rewrite in_app_iff. left. clear Hin. solve_In. auto.
-            } simpl in *.
-            assert (x5 = i2); subst.
-            { clear - Hin1 Hin' Hnd. inv Hin'. simpl_In; subst.
-              unfold idcaus_of_senv in Hnd. simpl_app.
-              apply NoDup_app_r, NoDup_app_r, NoDup_app_r, NoDup_app_l in Hnd.
-              eapply NoDup_snd_det; eauto. solve_In; simpl; eauto. clear Hin. solve_In; simpl; auto.
-            } clear Hin'.
-            eapply sem_var_det in Hv'1; eauto. eapply sem_var_det in Hv'2; eauto. rewrite Hv'1, Hv'2.
-            { eapply fby_det_Sn; eauto.
-              - simpl_Forall.
-                eapply det_exp_S with (k:=0) in He1; eauto. specialize (He1 He2). simpl in *; eauto.
-                + intros. eapply det_var_inv_local with (Hl1:=Hl1); eauto.
-                  intros * Hin'. apply idcaus_of_senv_In in Hin'.
-                  eapply Forall_forall in H22; eauto. eauto.
-                + rewrite <-length_typeof_numstreams, H1; auto.
-                + intros * IsF. eapply det_var_inv_local with (Hl1:=Hl1); eauto.
-                  * intros. eapply HSn; eauto.
-                    eapply DepOnLocal2; eauto. solve_Exists; split; auto.
-                  * intros * Hin'. apply idcaus_of_senv_In in Hin'.
-                    eapply Forall_forall in H23; eauto. eapply H23.
-                    eapply HenvS; simpl.
-                    { eapply idcaus_of_locals_In_local2 in Hin'; eauto. solve_In. }
-                    eapply DepOnLocal2; eauto. solve_Exists; split; auto.
-              - eapply Forall_forall in H22. 2:unfold idcaus_of_senv; simpl_app; apply in_app_iff, or_introl; solve_In.
-                simpl in *.
-                edestruct H22 as (Hinv&_). eapply Hinv; eauto. econstructor; solve_In. auto.
-            }
-
-        + (* deeper *)
-          econstructor; eauto.
-          * apply Forall_forall; intros * Hinblk.
-            destruct (in_dec ident_eq_dec cy (map snd (idcaus_of_locals x))). unfold idcaus_of_locals in i; simpl in i.
-            2:simpl_Forall; eapply sem_block_det_cons_nIn; eauto.
-            simpl_In.
-            inv_VarsDefined. rewrite Forall_forall in H.
-            { eapply H with (Γ:=Γ ++ senv_of_locs locs); eauto.
-              - clear - Hinblk Hnd.
-                eapply NoDup_locals_inv; eauto. rewrite idcaus_of_senv_app.
-                simpl_app; auto.
-              - simpl_Forall. now rewrite map_app, map_fst_senv_of_locs.
-              - rewrite map_app, map_fst_senv_of_locs.
-                etransitivity; eauto using incl_concat.
-                rewrite <-H7, Permutation_app_comm.
-                apply incl_app; [apply incl_appl|apply incl_appr]; eauto using incl_refl.
-              - intros * Hin'. inv Hin'.
-                apply in_app_iff in H0 as [|]; simpl_In; subst.
-                + eapply Env.In_refines; eauto with senv.
-                + destruct o as [(?&?)|]; simpl in *; try congruence.
-                  edestruct H15 as (?&?&?&?&?&?&?); eauto using sem_var_In.
-              - intros * Hin'. inv Hin'.
-                apply in_app_iff in H0 as [|]; simpl_In; subst.
-                + eapply Env.In_refines; eauto with senv.
-                + destruct o as [(?&?)|]; simpl in *; try congruence.
-                  edestruct H16 as (?&?&?&?&?&?&?); eauto using sem_var_In.
-              - intros * _. eapply det_var_inv_local with (Hl1:=Hl1); eauto.
-                intros * Hin'. eapply Forall_forall in H22; eauto.
-                clear - Hin'. unfold idcaus_of_senv. simpl_app. rewrite in_app_iff; auto.
-                destruct Hin' as [Hin'|Hin']; inv Hin'; simpl_In; [left|right]; solve_In. auto.
-              - simpl_Forall; auto.
-              - simpl_Forall; auto.
-              - intros * _ Hdep. eapply det_var_inv_local with (Hl1:=Hl1); eauto.
-                + intros. eapply HSn; eauto.
-                  econstructor; eauto. solve_Exists.
-                + intros * Hin'.
-                  assert (In cx (map snd (idcaus_of_senv (senv_of_locs locs)))) as Hin2.
-                  { apply idcaus_of_senv_In in Hin'. solve_In. }
-                  eapply Forall_forall with (x:=cx) in H23; eauto. eapply H23.
-                  eapply HenvS.
-                  * clear - Hin2. simpl_In. eapply idcaus_of_locals_In_local2 in Hin; solve_In.
-                  * econstructor; eauto. solve_Exists.
-              - intros * Hin' Hdep. apply HenvS.
-                + simpl_app. apply in_or_app, or_intror. solve_In.
-                + econstructor; eauto. solve_Exists.
-            }
-          * simpl_Forall. destruct H1; subst; eauto.
-            exfalso. clear - Hinenv H0 Hnd.
-            unfold idcaus_of_senv in *. simpl_app.
-            repeat rewrite map_map in Hnd. apply NoDup_app_r, NoDup_app_r in Hnd.
-            rewrite app_assoc in Hnd. eapply NoDup_app_In in Hnd.
-            eapply Hnd. solve_In. simpl.
-            rewrite in_app_iff in *. destruct H0 as [|]; [left|right]; solve_In. auto.
-    Qed.
-
-    Lemma det_vars_n :
-      forall nd n Hi1 Hi2 bs1 bs2,
-        det_nodes G ->
-        wt_node G nd ->
-        node_causal nd ->
-        EqStN n bs1 bs2 ->
-        sem_block G Hi1 bs1 (n_block nd) ->
-        sem_block G Hi2 bs2 (n_block nd) ->
-        Forall (det_var_inv (senv_of_inout (n_in nd ++ n_out nd)) n Hi1 Hi2) (map snd (idcaus (n_in nd))) ->
-        Forall (det_var_inv (senv_of_inout (n_in nd ++ n_out nd)) n Hi1 Hi2) (map snd (idcaus (n_in nd ++ n_out nd))).
-    Proof.
-      intros * HdetG Hwtn Hcaus Hbs Hsem1 Hsem2 Hins.
-
-      assert (sem_block_det n (map snd (idcaus (n_in nd ++ n_out nd) ++ idcaus_of_locals (n_block nd)))
-                            Hi1 Hi2 bs1 bs2 (n_block nd) /\
-              Forall (fun x => In x (map snd (idcaus (n_in nd ++ n_out nd))) ->
-                            det_var_inv (senv_of_inout (n_in nd ++ n_out nd)) n Hi1 Hi2 x)
-                     (map snd (idcaus (n_in nd ++ n_out nd) ++ idcaus_of_locals (n_block nd)))) as (_&Hvars).
-      2:{ eapply Forall_impl_In; [|eapply Forall_incl; [eapply Hvars|]]; eauto.
-          repeat rewrite idcaus_app. solve_incl_app. }
-
-      induction n.
-      - (* everyone is equal up to 0 anyway *)
-        split.
-        + eapply sem_block_det_0; eauto.
-        + eapply Forall_forall. intros ??????. split; intros; constructor.
-      - (* use the causal induction to step once *)
-        clear Hsem1 Hsem2.
-        destruct IHn as (Hblk&Hvars); eauto using EqStN_weaken.
-        { eapply Forall_impl; [|eapply Hins]; intros ?????.
-          split; intros Hin Hv1 Hv2; eapply EqStN_weaken; eauto.
-          1,2:eapply H in Hv1; eauto.
-        }
-
-        eapply node_causal_ind; eauto.
-        + intros ?? Hperm (Hblk'&Hvars'). split.
-          * eapply sem_block_det_Perm; eauto.
-          * rewrite <-Hperm; auto.
-        + split; auto.
-          eapply sem_block_det_S; [|eauto]. solve_incl_app.
-        + intros * Hin (Hblk'&Hvars') Hdep.
-          repeat rewrite idcaus_app, map_app, in_app_iff in Hin.
-          destruct Hcaus as (Hnd&_).
-          destruct Hin as [[Hin|Hin]|Hin]; (split; [|constructor; auto; intros Hin']).
-          * eapply sem_block_det_cons_nIn; eauto.
-            intros Hin'. clear - Hin Hin' Hnd. simpl_app.
-            eapply NoDup_app_In in Hnd; eauto. eapply Hnd.
-            repeat rewrite in_app_iff in *. auto.
-          * eapply Forall_forall in Hins; eauto.
-          * eapply sem_block_det_cons_nIn; eauto.
-            intros Hin'. clear - Hin Hin' Hnd. simpl_app.
-            eapply NoDup_app_r, NoDup_app_In in Hnd; eauto.
-          * pose proof (n_defd nd) as (?&Hdef&Hperm). simpl_In.
-            eapply det_block_S; eauto.
-            -- clear - Hnd. now rewrite idcaus_of_senv_inout.
-            -- rewrite map_fst_senv_of_inout. apply node_NoDupLocals.
-            -- rewrite map_fst_senv_of_inout, Hperm. solve_incl_app.
-            -- intros * Has. inv Has. simpl_In. congruence.
-            -- intros * Has. inv Has. simpl_In. congruence.
-            -- intros * [Hin'|Hin']; inv Hin'; simpl_In; try congruence.
-               eapply Forall_forall in Hvars; eauto. eapply Hvars. solve_In.
-               rewrite map_app. apply in_app_iff, or_introl. solve_In.
-            -- destruct Hwtn as (?&?&?&?); auto.
-            -- rewrite Hperm. solve_In.
-            -- clear - Hin0. econstructor. solve_In; eauto using in_or_app.
-               1,2:simpl; auto.
-            -- intros * [Hin'|Hin'] ?; inv Hin'; simpl_In; try congruence.
-               eapply Forall_forall in Hvars'; eauto. eapply Hvars'. solve_In.
-          * pose proof (n_defd nd) as (?&Hdef&Hperm).
-            simpl_In.
-            eapply sem_block_det_cons_In; eauto.
-            -- clear - Hnd. now rewrite idcaus_of_senv_inout.
-            -- rewrite map_fst_senv_of_inout. apply node_NoDupLocals.
-            -- rewrite map_fst_senv_of_inout, Hperm. solve_incl_app.
-            -- intros * Has. inv Has. simpl_In. congruence.
-            -- intros * Has. inv Has. simpl_In. congruence.
-            -- intros * [Hin'|Hin']; inv Hin'; simpl_In; try congruence.
-               eapply Forall_forall in Hvars; eauto. eapply Hvars. solve_In.
-               rewrite map_app. apply in_app_iff, or_introl. solve_In.
-            -- destruct Hwtn as (?&?&?&?); auto.
-            -- intros * [Hin'|Hin'] ?; inv Hin'; simpl_In; try congruence.
-               eapply Forall_forall in Hvars'; eauto. eapply Hvars'. solve_In.
-          * exfalso. rewrite map_app in Hnd.
-            eapply NoDup_app_In in Hnd; eauto.
-    Qed.
-
-  End sem_block_det.
-
-  Lemma det_global_n {PSyn prefs} : forall (G : @global PSyn prefs),
-      wt_global G ->
-      Forall node_causal (nodes G) ->
-      det_nodes G.
+  Lemma P_vars_S :
+    forall n env xs,
+      P_vars (S n) env xs ->
+      P_vars n env xs.
   Proof.
-    intros (enms&nds).
-    induction nds as [|nd nds]; intros Hwt Hcaus ?????? Heqins Hs1 Hs2;
-      inv Hcaus. now inv Hs1.
-    inversion_clear Hs1 as [?????? Hfind1 Hins1 Houts1 Hbcks1 Hbk1].
-    inversion_clear Hs2 as [?????? Hfind2 Hins2 Houts2 Hbcks2 Hbk2].
-    rewrite Hfind1 in Hfind2. inv Hfind2.
-    destruct (ident_eq_dec (n_name nd) f); subst.
-    - assert (Hfind2:=Hfind1). rewrite find_node_now in Hfind2; auto; inv Hfind2.
-      assert (~ Is_node_in_block (n_name n1) (n_block n1)) as Hnin.
-      { eapply find_node_not_Is_node_in; eauto using wl_global_Ordered_nodes with ltyping. }
-      eapply sem_block_cons in Hbcks1; eauto using wl_global_Ordered_nodes with ltyping.
-      eapply sem_block_cons in Hbcks2; eauto using wl_global_Ordered_nodes with ltyping.
-
-      assert (Forall (det_var_inv (senv_of_inout (n_in n1 ++ n_out n1)) n (H, @Env.empty _) (H0, @Env.empty _)) (map snd (idcaus (n_in n1)))) as Hins.
-      { eapply node_causal_NoDup in H1 as Hnd.
-        clear - Heqins Hins1 Hins2 Hnd.
-        assert (incl (idcaus (n_in n1)) (idcaus (n_in n1 ++ n_out n1))) as Hincl.
-        { rewrite idcaus_app. solve_incl_app. }
-        revert ins1 ins2 Hins1 Hins2 Heqins Hnd Hincl.
-        generalize (n_in n1 ++ n_out n1) as cenv.
-        induction (n_in n1) as [|(?&(?&?)&?)]; intros * Hins1 Hins2 Heqins;
-          inv Hins1; inv Hins2; inv Heqins; constructor; eauto; simpl in *.
-        - intros ???. split; intros Hin Hv1 Hv2; inv Hin; simpl_In; try congruence.
-          specialize (Hincl _ (in_eq _ _)).
-          eapply NoDup_snd_det in Hincl; [|eauto|solve_In]; subst.
-          eapply sem_var_det in H3; eauto. eapply sem_var_det in H4; eauto.
-          now rewrite H3, H4.
-        - eapply IHl; eauto. eapply incl_cons'; eauto. }
-      eapply det_vars_n in Hins; eauto.
-      + eapply Forall2_trans_ex in Houts2; [|eapply Forall2_swap_args, Houts1].
-        eapply Forall2_impl_In; [|eauto]; intros ?? _ _ (?&Hin&Hv1&Hv2). simpl_In.
-        unfold idcaus in Hins. rewrite Forall_map, Forall_map in Hins.
-        eapply Forall_forall in Hins; [|eauto using in_or_app].
-        eapply Hins in Hv2; eauto; simpl in *.
-        econstructor. solve_In; eauto using in_or_app. 1,2:reflexivity.
-      + inv Hwt; inv H4. eapply IHnds; eauto. split; eauto.
-      + inv Hwt; inv H4. destruct H7; auto.
-      + eapply clocks_of_EqStN; eauto.
-    - rewrite find_node_other in Hfind1; auto.
-      eapply IHnds; eauto. inv Hwt; inv H4; split; auto.
-      1,2:econstructor; eauto.
-      1,2:eapply sem_block_cons; eauto using wl_global_Ordered_nodes with ltyping.
-      1,2:eapply find_node_later_not_Is_node_in; eauto using wl_global_Ordered_nodes with ltyping.
+    unfold P_vars.
+    eauto using Forall_impl, P_var_S.
   Qed.
 
-  Theorem det_global {PSyn prefs} : forall (G: @global PSyn prefs) f ins outs1 outs2,
-      wt_global G ->
-      Forall node_causal (nodes G) ->
-      sem_node G f ins outs1 ->
-      sem_node G f ins outs2 ->
-      EqSts outs1 outs2.
+  Lemma P_vars_weaken :
+    forall n env xs ys,
+      P_vars n env (xs ++ ys) ->
+      P_vars n env ys.
   Proof.
-    intros * Hwt Hcaus Hsem1 Hsem2.
-    eapply det_nodes_ins; eauto.
-    eapply det_global_n; eauto.
+    unfold P_vars.
+    eauto using Forall_app_weaken.
   Qed.
 
-End LSEMDETERMINISM.
+  (* TODO: move to LSyntax *)
+  Lemma annots_numstreams :
+    forall es, length (annots es) = list_sum (map numstreams es).
+  Proof.
+    induction es; simpl; auto.
+    rewrite app_length; f_equal; auto.
+    rewrite <- length_typeof_numstreams, typeof_annot.
+    now rewrite map_length.
+  Qed.
 
-Module LSemDeterminismFun
+  (* TODO: move? *)
+  Lemma denot_equation_input :
+    forall {PSyn prefs} (G : @global PSyn prefs) Γ
+      e ins envI bs env x,
+      wt_equation G Γ e ->
+      In x ins ->
+      denot_equation ins e envI bs env x = envI x.
+  Proof.
+    intros * Hwt Hx.
+    apply mem_ident_spec in Hx.
+    destruct e as (xs,es).
+    destruct Hwt as [? Hwt]. apply Forall2_length in Hwt.
+    rewrite length_typesof_annots, annots_numstreams in Hwt.
+    rewrite denot_equation_eq.
+    cases_eqn HH; congruence.
+  Qed.
+
+  Lemma P_var_input :
+    forall {PSyn prefs} (G : @global PSyn prefs) nd envI bs x n,
+      restr_node nd ->
+      wt_node G nd ->
+      In x (map fst (n_in nd)) ->
+      P_vars n envI (map fst (n_in nd)) ->
+      P_var n (FIXP (DS_prod SI) (denot_node nd envI bs)) x.
+  Proof.
+    intros * Hr Hwt Hx Hins.
+    unfold P_vars, P_var in *.
+    rewrite FIXP_eq, PROJ_simpl.
+    unfold denot_node, denot_block.
+    destruct Hwt as (?&?&?& Hwt).
+    destruct Hr. inv Hwt.
+    erewrite denot_equation_input, Forall_forall, <- PROJ_simpl in *; eauto.
+  Qed.
+
+  Lemma P_exps_k : forall n es ins envI bs env k,
+      P_exps (P_exp n ins envI bs env) es k ->
+      is_cons (nrem n (get_nth (denot_exps ins es envI bs env) k)).
+  Proof.
+    induction es as [| e es]; intros * Hp (* Hwl Hr *); inv Hp; simpl_Forall.
+    - setoid_rewrite denot_exps_eq.
+      setoid_rewrite nprod_app_nth1; eauto using Is_free_left_list.
+    - setoid_rewrite denot_exps_eq.
+      setoid_rewrite nprod_app_nth2; eauto using Is_free_left_list.
+  Qed.
+
+  (* TODO: move? *)
+  Lemma P_exps_impl :
+    forall (Q_exp P_exp : exp -> nat -> Prop) es k,
+      P_exps Q_exp es k ->
+      P_exps (fun e k => Q_exp e k -> P_exp e k) es k ->
+      P_exps P_exp es k.
+  Proof.
+    intros * Hpq Hq.
+    induction Hpq; inv Hq; constructor; auto; lia.
+  Qed.
+
+  (* TODO: move? *)
+  Lemma P_exps_Forall :
+    forall (P_exp : exp -> Prop) es k,
+      Forall P_exp es ->
+      k < list_sum (map numstreams es) ->
+      P_exps (fun e _ => P_exp e) es k.
+  Proof.
+    induction es as [|e es]; simpl; intros * Hf Hk. inv Hk.
+    inv Hf.
+    destruct (Nat.lt_ge_cases k (numstreams e)); auto using P_exps.
+    constructor 2; auto.
+    apply IHes; auto; lia.
+  Qed.
+
+  Lemma exp_O :
+    forall Γ e ins envI bs env k,
+      is_cons (nrem O bs) ->
+      P_vars O envI ins ->
+      k < numstreams e ->
+      (forall x, Is_free_left Γ x k e -> P_var O env x) ->
+      wl_exp G e ->
+      wx_exp Γ e ->
+      restr_exp e ->
+      P_exp O ins envI bs env e k.
+  Proof.
+    intros * Hbs Hins Hk Hdep Hwl Hwx Hre.
+    assert (Hwl' := Hwl).
+    revert Hwl Hre.
+    eapply exp_causal_ind with (15 := Hdep); eauto.
+    all: intros; clear dependent e; inv Hre; unfold P_exp.
+    - (* const *)
+      rewrite denot_exp_eq.
+      now apply is_consn_sconst.
+    - (* var *)
+      rewrite denot_exp_eq.
+      unfold P_vars, P_var in *.
+      simpl. rewrite ID_simpl, Id_simpl, Forall_forall in *.
+      cases_eqn HH.
+      + (* in *)
+        rewrite mem_ident_spec in HH.
+        now apply Hins.
+      + (* out *)
+        apply HasCausInj in H; subst; auto.
+    - (* unop *)
+      rewrite denot_exp_eq.
+      cases_eqn HH; subst.
+      1,3: inv Hwl; rewrite <- length_typeof_numstreams, HH in *; now simpl in *.
+      assert (is_cons (nrem O (get_nth (denot_exp ins e1 envI bs env0) 0))) as He.
+      { inv Hwl. apply H; auto. }
+      revert He.
+      generalize (denot_exp ins e1 envI bs env0).
+      generalize (numstreams e1).
+      simpl. intros; cases.
+      2: apply is_consn_DS_const with (n := O). (* pourquoi auto ne fonctionne pas ? *)
+      apply is_consn_sunop with (n := O); auto.
+    - (* fby *)
+      rewrite denot_exp_eq; simpl.
+      unfold eq_rect_r, eq_rect.
+      cases.
+      2,3: rewrite get_nth_const; auto; apply (is_consn_DS_const _ O).
+      rewrite lift2_nth; auto; cases.
+      apply is_cons_fby; auto.
+      inv Hwl.
+      rewrite annots_numstreams, H10, <- H9 in *.
+      eapply P_exps_k with (n := O); eauto.
+      eauto using P_exps_impl, P_exps_Forall.
+  Qed.
+
+  Lemma exp_n :
+    forall Γ n e ins envI bs env k,
+      is_cons (nrem n bs) ->
+      P_vars n envI ins ->
+      k < numstreams e ->
+      wl_exp G e ->
+      wx_exp Γ e ->
+      restr_exp e ->
+      (forall x cx, HasCaus Γ x cx -> P_var n env cx) ->
+      P_exp n ins envI bs env e k.
+  Proof.
+    intros ?????? env ? Hbs Hins.
+    revert k.
+    induction e using exp_ind2; simpl; intros ? Hk Hwl Hwx Hre Hn.
+    all: inv Hre; unfold P_exp.
+    - (* const *)
+      assert (k = O) by lia; subst.
+      rewrite denot_exp_eq.
+      now apply is_consn_sconst.
+    - (* var *)
+      assert (k = O) by lia; subst.
+      unfold P_vars, P_var in *.
+      simpl. rewrite ID_simpl, Id_simpl, Forall_forall in *.
+      setoid_rewrite denot_exp_eq.
+      cases_eqn HH.
+      + (* in *)
+        rewrite mem_ident_spec in HH.
+        now apply Hins.
+      + (* out *)
+        inv Hwx.
+        eapply Hn, HasCausRefl; auto.
+    - (* unop *)
+      assert (k = O) by lia; subst.
+      rewrite denot_exp_eq.
+      cases_eqn HH; subst.
+      1,3: inv Hwl; rewrite <- length_typeof_numstreams, HH in *; now simpl in *.
+      assert (is_cons (nrem n (get_nth (denot_exp ins e envI bs env) 0))) as He.
+      { inv Hwl. inv Hwx. eapply IHe; auto; lia. }
+      revert He.
+      generalize (denot_exp ins e envI bs env).
+      generalize (numstreams e).
+      intros; cases.
+      2: apply is_consn_DS_const. (* pourquoi auto ne fonctionne pas ? *)
+      apply is_consn_sunop; auto.
+    - (* fby *)
+      rewrite denot_exp_eq; simpl.
+      unfold eq_rect_r, eq_rect.
+      cases.
+      2,3: rewrite get_nth_const; auto; apply (is_consn_DS_const _ n).
+      rewrite lift2_nth; auto; cases.
+      inv Hwl.
+      apply is_consn_fby.
+      (* TODO: factoriser un peu le raisonnement *)
+      + (* e0s *)
+        assert (k < list_sum (map numstreams e0s))
+          by (rewrite annots_numstreams in *; congruence).
+        apply P_exps_k.
+        inv Hwx. clear dependent es. clear H9.
+        revert dependent k. induction e0s; intros; simpl in *. lia.
+        simpl_Forall.
+        destruct (Nat.lt_ge_cases k (numstreams a0)); auto using P_exps.
+        constructor 2; auto. apply IHe0s; auto; lia.
+      + (* es *)
+        assert (k < list_sum (map numstreams es))
+          by (rewrite annots_numstreams in *; congruence).
+        apply P_exps_k.
+        inv Hwx. clear dependent e0s. clear H10.
+        revert dependent k. induction es; intros; simpl in *. lia.
+        simpl_Forall.
+        destruct (Nat.lt_ge_cases k (numstreams a0)); auto using P_exps.
+        constructor 2; auto. apply IHes; auto; lia.
+  Qed.
+
+  Lemma exps_n :
+    forall Γ n es ins envI bs env k,
+      is_cons (nrem n bs) ->
+      P_vars n envI ins ->
+      k < list_sum (map numstreams es) ->
+      Forall (wl_exp G) es ->
+      Forall (wx_exp Γ) es ->
+      Forall restr_exp es ->
+      (forall x cx, HasCaus Γ x cx -> P_var n env cx) ->
+      P_exps (P_exp n ins envI bs env) es k.
+  Proof.
+    induction es as [| e es]; simpl; intros * Hbs Hins Hk Hwl Hwx Hre Hn.
+    inv Hk.
+    simpl_Forall.
+    destruct (Nat.lt_ge_cases k (numstreams e)).
+    - constructor; eauto using exp_n.
+    - constructor 2; auto. apply IHes; auto; lia.
+  Qed.
+
+  Lemma exp_S :
+    forall Γ n e ins envI bs env k,
+      is_cons (nrem (S n) bs) ->
+      P_vars (S n) envI ins ->
+      k < numstreams e ->
+      (forall x, Is_free_left Γ x k e -> P_var (S n) env x) ->
+      wl_exp G e ->
+      wx_exp Γ e ->
+      restr_exp e ->
+      (forall x cx, HasCaus Γ x cx -> P_var n env cx) ->
+      P_exp (S n) ins envI bs env e k.
+  Proof.
+    intros ?????? env ? Hbs Hins Hk Hdep Hwl Hwx Hre Hn.
+    assert (Hwl' := Hwl).
+    assert (Hwx' := Hwx).
+    revert Hwl Hwx Hre.
+    eapply exp_causal_ind with (15 := Hdep); eauto.
+    all: clear dependent e; clear k.
+    all: intros; inv Hre; unfold P_exp.
+    - (* const *)
+      rewrite denot_exp_eq.
+      now apply is_consn_sconst.
+    - (* var *)
+      unfold P_vars, P_var in *.
+      simpl. rewrite ID_simpl, Id_simpl, Forall_forall in *.
+      setoid_rewrite denot_exp_eq.
+      cases_eqn HH.
+      + (* in *)
+        rewrite mem_ident_spec in HH.
+        now apply Hins.
+      + (* out *)
+        apply HasCausInj in H; subst; auto.
+    - (* unop *)
+      rewrite denot_exp_eq.
+      cases_eqn HH; subst.
+      1,3: inv Hwl; rewrite <- length_typeof_numstreams, HH in *; now simpl in *.
+      assert (is_cons (nrem (S n) (get_nth (denot_exp ins e1 envI bs env) 0))) as He.
+      { inv Hwl. inv Hwx. apply H; auto. }
+      revert He.
+      generalize (denot_exp ins e1 envI bs env).
+      generalize (numstreams e1).
+      intros; cases.
+      2: apply is_consn_DS_const. (* pourquoi auto ne fonctionne pas ? *)
+      apply is_consn_sunop; auto.
+    - (* fby *)
+      rewrite denot_exp_eq; simpl.
+      unfold eq_rect_r, eq_rect.
+      cases.
+      2,3: rewrite get_nth_const; auto; apply (is_consn_DS_const _ (S n)).
+      rewrite lift2_nth; auto; cases.
+      inv Hwl. inv Hwx.
+      apply is_consn_S_fby.
+      + (* e0s *)
+        assert (k < list_sum (map numstreams e0s))
+          by (rewrite annots_numstreams in *; congruence).
+        do 3 (apply P_exps_impl in H0; eauto using P_exps_Forall).
+        now apply P_exps_k.
+      + (* es *)
+        eapply P_exps_k, exps_n; eauto using is_consn_S, P_vars_S.
+  Qed.
+
+  (* TODO: move, rename *)
+  Lemma P_var_input' :
+    forall Γ ins envI bs e x n,
+      wt_equation G Γ e ->
+      In x ins ->
+      P_vars n envI ins ->
+      P_var n (FIXP (DS_prod SI) (denot_equation ins e envI bs)) x.
+  Proof.
+    intros * Hwt Hin Hins.
+    unfold P_vars, P_var in *.
+    rewrite FIXP_eq, PROJ_simpl.
+    erewrite denot_equation_input, Forall_forall, <- PROJ_simpl in *; eauto.
+  Qed.
+
+  Lemma equation_n :
+    forall xs es n k ins envI bs,
+      let env := FIXP (DS_prod SI) (denot_equation ins (xs,es) envI bs) in
+      NoDup (ins ++ xs) ->
+      k < length xs ->
+      P_exps (P_exp n ins envI bs env) es k ->
+      P_var n env (nth k xs xH).
+  Proof.
+    intros ??????? env Hnd Hk Hes.
+    subst env.
+    unfold P_var.
+    rewrite FIXP_eq, PROJ_simpl, denot_equation_eq.
+    rewrite mem_nth_nth; eauto using NoDup_app_r.
+    cases_eqn HH; auto using is_consn_DS_const, P_exps_k.
+    (* cas pénible *)
+    exfalso. rewrite mem_ident_spec in *.
+    eapply NoDup_app_In; eauto using nth_In.
+  Qed.
+
+  Lemma denot_S :
+    forall nd envI bs n,
+      restr_node nd ->
+      wt_node G nd ->
+      node_causal nd ->
+      is_cons (nrem (S n) bs) ->
+      P_vars (S n) envI (map fst nd.(n_in)) ->
+      P_vars n (FIXP _ (denot_node nd envI bs)) (map fst nd.(n_out)) ->
+      P_vars (S n) (FIXP _ (denot_node nd envI bs)) (map fst nd.(n_out)).
+  Proof.
+    intros * Hr Hwt Hcaus Hbs Hins Hn.
+    eapply P_vars_weaken.
+    rewrite <- map_app, <- idcaus_map.
+    rewrite <- (@app_nil_r (ident*ident)) at 1.
+    assert (idcaus_of_locals (n_block nd) = []) as <- by now inv Hr.
+    eapply node_causal_ind; auto.
+    - unfold P_vars. now intros ?? ->.
+    - now red.
+    - intros x xs' [Hx|Hx] Hxs' Hdep.
+      2: now destruct Hr; simpl in *.
+      constructor; auto.
+      rewrite idcaus_app, map_app, in_app_iff, 2 idcaus_map in Hx.
+      destruct Hx as [|Hx]; eauto using P_var_input.
+      (* TODO: nettoyer *)
+
+      destruct (n_defd nd) as (ys & Hvd & Hperm).
+      destruct Hwt as (?&?&?& Hwt).
+      unfold denot_node, denot_block in *.
+      inv Hvd; destruct Hr as [? es Hr]; try congruence.
+      inv H3; simpl (fst _) in *.
+
+      rewrite <- Hperm in Hx.
+      apply In_nth with (d := xH) in Hx as (k & Hlen & Hnth); subst.
+      eapply equation_n; eauto.
+      { rewrite Hperm, <- map_app; apply node_NoDup. }
+      eapply Pexp_Pexps with
+        (Γ := (senv_of_inout (n_in nd ++ n_out nd)))
+        (P_var := P_var (S n) (FIXP _ (denot_equation (map fst (n_in nd)) (xs, es) envI bs))); eauto.
+      + inv Hwt.  assert(Wte := H4). destruct H4 as [Hwt].
+        apply Forall_wt_exp_wx_exp in Hwt as Hwx.
+        apply Forall_wt_exp_wl_exp in Hwt as Hwl.
+        apply Forall_forall.
+        intros e Hin k' Hk' Hdp.
+        pose proof (Forall_In _ _ _ Hwx Hin) as Hwxe.
+        pose proof (Forall_In _ _ _ Hwl Hin) as Hwle.
+        pose proof (Forall_In _ _ _ Hwt Hin) as Hwte.
+        pose proof (Forall_In _ _ _ Hr  Hin) as Hre.
+        eapply exp_S; eauto.
+        (* TODO: lemma pour ça : *)
+        intros x cx Hc.
+        apply HasCausInj in Hc as ?; subst.
+        eapply or_introl, idcaus_of_senv_In in Hc.
+        rewrite idcaus_of_senv_inout in Hc.
+        apply In_list_pair_l in Hc.
+        rewrite map_fst_idcaus, map_app, in_app_iff in Hc.
+        destruct Hc as [Hc|]; eauto using P_vars_In, P_var_input', P_vars_S.
+      + intros x Hfr.
+        eapply P_vars_In; eauto.
+        apply Hdep.
+        econstructor; eauto using (nth_error_nth' _ xH).
+        apply HasCausRefl.
+        (* TODO: lemme pour ça ? : *)
+        rewrite <- map_fst_senv_of_inout in Hperm.
+        unfold senv_of_inout in *.
+        constructor.
+        rewrite fst_InMembers, 2 map_app, in_app, <- Hperm.
+        auto using nth_In.
+      + inv Hwt.
+        destruct H4 as [? Hwt]. apply Forall2_length in Hwt.
+        rewrite length_typesof_annots in Hwt. congruence.
+  Qed.
+
+  (* TODO: ressemble beaucoup à denot_S... *)
+  Lemma denot_O :
+    forall nd envI bs,
+      restr_node nd ->
+      wt_node G nd ->
+      node_causal nd ->
+      is_cons (nrem O bs) ->
+      P_vars O envI (map fst nd.(n_in)) ->
+      P_vars O (FIXP _ (denot_node nd envI bs)) (map fst nd.(n_out)).
+  Proof.
+    intros * Hr Hwt Hcaus Hbs Hins.
+    eapply P_vars_weaken.
+    rewrite <- map_app, <- idcaus_map.
+    rewrite <- (@app_nil_r (ident*ident)) at 1.
+    assert (idcaus_of_locals (n_block nd) = []) as <- by now inv Hr.
+    eapply node_causal_ind; auto.
+    - unfold P_vars. now intros ?? ->.
+    - now red.
+    - intros x xs' [Hx|Hx] Hxs' Hdep.
+      2: now destruct Hr; simpl in *.
+      constructor; auto.
+      rewrite idcaus_app, map_app, in_app_iff, 2 idcaus_map in Hx.
+      destruct Hx as [|Hx]; eauto using P_var_input.
+
+      destruct (n_defd nd) as (ys & Hvd & Hperm).
+      destruct Hwt as (?&?&?& Hwt).
+      unfold denot_node, denot_block in *.
+      inv Hvd; destruct Hr as [? es Hr]; try congruence.
+      inv H3; simpl (fst _) in *.
+
+      rewrite <- Hperm in Hx.
+      apply In_nth with (d := xH) in Hx as (k & Hlen & Hnth); subst.
+      eapply equation_n; eauto.
+      { rewrite Hperm, <- map_app; apply node_NoDup. }
+      eapply Pexp_Pexps with
+        (Γ := (senv_of_inout (n_in nd ++ n_out nd)))
+        (P_var := P_var O (FIXP _ (denot_equation (map fst (n_in nd)) (xs, es) envI bs))); eauto.
+      + inv Hwt. assert(Wte := H4). destruct H4 as [Hwt].
+        apply Forall_wt_exp_wx_exp in Hwt as Hwx.
+        apply Forall_wt_exp_wl_exp in Hwt as Hwl.
+        apply Forall_forall.
+        intros e Hin k' Hk' Hdp.
+        pose proof (Forall_In _ _ _ Hwx Hin) as Hwxe.
+        pose proof (Forall_In _ _ _ Hwl Hin) as Hwle.
+        pose proof (Forall_In _ _ _ Hwt Hin) as Hwte.
+        pose proof (Forall_In _ _ _ Hr  Hin) as Hre.
+        eapply exp_O; eauto.
+      + intros x Hfr.
+        eapply P_vars_In; eauto.
+        apply Hdep.
+        econstructor; eauto using (nth_error_nth' _ xH).
+        apply HasCausRefl.
+        (* TODO: lemme pour ça ? : *)
+        rewrite <- map_fst_senv_of_inout in Hperm.
+        unfold senv_of_inout in *.
+        constructor.
+        rewrite fst_InMembers, 2 map_app, in_app, <- Hperm.
+        auto using nth_In.
+      + inv Hwt.
+        destruct H4 as [? Hwt]. apply Forall2_length in Hwt.
+        rewrite length_typesof_annots in Hwt. congruence.
+  Qed.
+
+  Theorem denot_n :
+    forall nd envI bs n,
+      restr_node nd ->
+      wt_node G nd ->
+      node_causal nd ->
+      is_cons (nrem n bs) ->
+      P_vars n envI (map fst nd.(n_in)) ->
+      P_vars n (FIXP _ (denot_node nd envI bs)) (map fst nd.(n_out)).
+  Proof.
+    induction n; intros Hr Hwt Hcaus Hbs Hins.
+    - apply denot_O; auto.
+    - apply denot_S; auto using is_consn_S, P_vars_S.
+  Qed.
+
+  (** Maintenant on passe à l'infini *)
+
+  Definition all_infinite (env : DS_prod SI) (l : list ident) : Prop :=
+    forall x, In x l -> infinite (env x).
+
+  Lemma infinite_P_vars :
+    forall l env, all_infinite env l <-> (forall n, P_vars n env l).
+  Proof.
+    intros l env.
+    unfold P_vars, P_var, all_infinite.
+    setoid_rewrite Forall_forall.
+    Opaque nrem. (* WTF *)
+    setoid_rewrite PROJ_simpl.
+    split; eauto using nrem_inf, inf_nrem.
+  Qed.
+
+  Theorem denot_inf :
+    forall nd envI bs,
+      restr_node nd ->
+      wt_node G nd ->
+      node_causal nd ->
+      infinite bs ->
+      all_infinite envI (map fst nd.(n_in)) ->
+      all_infinite (FIXP _ (denot_node nd envI bs)) (map fst nd.(n_out)).
+  Proof.
+    intros.
+    rewrite infinite_P_vars in *.
+    intro.
+    eapply denot_n; eauto using inf_nrem.
+  Qed.
+
+  End node_inf.
+
+End LDENOTINF.
+
+Module LDenotInfFun
        (Ids   : IDS)
        (Op    : OPERATORS)
        (OpAux : OPERATORS_AUX Ids Op)
@@ -1676,7 +653,7 @@ Module LSemDeterminismFun
        (LCA   : LCAUSALITY Ids Op OpAux Cks Senv Syn)
        (Lord  : LORDERED Ids Op OpAux Cks Senv Syn)
        (CStr  : COINDSTREAMS Ids Op OpAux Cks)
-       (Sem   : LSEMANTICS Ids Op OpAux Cks Senv Syn Lord CStr)
-<: LSEMDETERMINISM Ids Op OpAux Cks Senv Syn Typ LCA Lord CStr Sem.
-  Include LSEMDETERMINISM Ids Op OpAux Cks Senv Syn Typ LCA Lord CStr Sem.
-End LSemDeterminismFun.
+       (Den   : LDENOT     Ids Op OpAux Cks Senv Syn Lord CStr)
+<: LDENOTINF Ids Op OpAux Cks Senv Syn Typ LCA Lord CStr Den.
+  Include LDENOTINF Ids Op OpAux Cks Senv Syn Typ LCA Lord CStr Den.
+End LDenotInfFun.
